AwsCryptographicMaterialProviders/src/AwsCryptographyMaterialProvidersOperations.dfy
@@ -1,0 +1,461 @@
+// Copyright Amazon.com Inc. or its affiliates. All Rights Reserved.
+// SPDX-License-Identifier: Apache-2.0
+include "../Model/AwsCryptographyMaterialProvidersTypes.dfy"
+
+include "Keyrings/AwsKms/StrictMultiKeyring.dfy"
+include "Keyrings/MultiKeyring.dfy"
+include "Keyrings/AwsKms/AwsKmsKeyring.dfy"
+include "Keyrings/AwsKms/AwsKmsUtils.dfy"
+include "Keyrings/AwsKms/AwsKmsDiscoveryKeyring.dfy"
+include "Keyrings/AwsKms/DiscoveryMultiKeyring.dfy"
+include "Keyrings/AwsKms/AwsKmsMrkKeyring.dfy"
+include "Keyrings/AwsKms/AwsKmsUtils.dfy"
+include "Keyrings/AwsKms/MrkAwareStrictMultiKeyring.dfy"
+include "Keyrings/AwsKms/AwsKmsMrkDiscoveryKeyring.dfy"
+include "Keyrings/AwsKms/MrkAwareDiscoveryMultiKeyring.dfy"
+include "Keyrings/RawAESKeyring.dfy"
+include "Keyrings/RawRSAKeyring.dfy"
+include "CMMs/DefaultCMM.dfy"
+include "DefaultClientSupplier.dfy"
+include "Materials.dfy"
+include "Commitment.dfy"
+include "AlgorithmSuites.dfy"
+
+module AwsCryptographyMaterialProvidersOperations refines AbstractAwsCryptographyMaterialProvidersOperations {
+
+  import MultiKeyring
+  import opened S = StrictMultiKeyring
+  import opened D = DiscoveryMultiKeyring
+  import opened MD = MrkAwareDiscoveryMultiKeyring
+  import opened M = MrkAwareStrictMultiKeyring
+  import AwsKmsKeyring
+  import AwsKmsMrkKeyring
+  import AwsKmsDiscoveryKeyring
+  import AwsKmsMrkDiscoveryKeyring
+  import RawAESKeyring
+  import RawRSAKeyring
+  import opened C = DefaultCMM
+  import Crypto = AwsCryptographyPrimitivesTypes
+  import Aws.Cryptography.Primitives
+  import opened AwsKmsUtils
+  import DefaultClientSupplier
+  import Materials
+  import Commitment
+  import AlgorithmSuites
+
+  datatype Config = Config(
+    nameonly crypto: Primitives.AtomicPrimitivesClient
+  )
+
+  type InternalConfig = Config
+
+  predicate ValidInternalConfig?(config: InternalConfig)
+  {
+    && config.crypto.ValidState()
+  }
+
+  function ModifiesInternalConfig(config: InternalConfig) : set<object>
+  {
+    config.crypto.Modifies
+  }
+
+  predicate CreateAwsKmsKeyringEnsuresPublicly(input: CreateAwsKmsKeyringInput, output: Result<IKeyring, Error>)
+  {true}
+
+  method CreateAwsKmsKeyring(config: InternalConfig, input: CreateAwsKmsKeyringInput)
+    returns (output: Result<IKeyring, Error>)
+  {
+    var _ :- ValidateKmsKeyId(input.kmsKeyId);
+    var grantTokens :- GetValidGrantTokens(input.grantTokens);
+    var keyring := new AwsKmsKeyring.AwsKmsKeyring(input.kmsClient, input.kmsKeyId, grantTokens);
+    return Success(keyring);
+  }
+
+  predicate CreateAwsKmsDiscoveryKeyringEnsuresPublicly(input: CreateAwsKmsDiscoveryKeyringInput, output: Result<IKeyring, Error>)
+  {true}
+
+  method CreateAwsKmsDiscoveryKeyring(config: InternalConfig, input: CreateAwsKmsDiscoveryKeyringInput)
+    returns (output: Result<IKeyring, Error>)
+  {
+    if input.discoveryFilter.Some? {
+      var _ :- ValidateDiscoveryFilter(input.discoveryFilter.value);
+    }
+    var grantTokens :- GetValidGrantTokens(input.grantTokens);
+    var keyring := new AwsKmsDiscoveryKeyring.AwsKmsDiscoveryKeyring(input.kmsClient, input.discoveryFilter, grantTokens);
+    return Success(keyring);
+  }
+
+  predicate CreateAwsKmsMultiKeyringEnsuresPublicly(input: CreateAwsKmsMultiKeyringInput, output: Result<IKeyring, Error>)
+  {true}
+
+  method CreateAwsKmsMultiKeyring(config: InternalConfig, input: CreateAwsKmsMultiKeyringInput)
+    returns (output: Result<IKeyring, Error>)
+  {
+    var grantTokens :- GetValidGrantTokens(input.grantTokens);
+
+    if input.clientSupplier.Some? {
+      output := StrictMultiKeyring(
+        input.generator,
+        input.kmsKeyIds,
+        input.clientSupplier.value,
+        Option.Some(grantTokens)
+      );
+    } else {
+      //= compliance/framework/aws-kms/aws-kms-multi-keyrings.txt#2.5
+      //# If a regional client supplier is not passed, then a default MUST be
+      //# created that takes a region string and generates a default AWS SDK
+      //# client for the given region.
+      var clientSupplier :- CreateDefaultClientSupplier(config, Types.CreateDefaultClientSupplierInput());
+      output := StrictMultiKeyring(
+        input.generator,
+        input.kmsKeyIds,
+        clientSupplier,
+        Option.Some(grantTokens)
+      );
+    }
+  }
+
+  predicate CreateAwsKmsDiscoveryMultiKeyringEnsuresPublicly(input: CreateAwsKmsDiscoveryMultiKeyringInput, output: Result<IKeyring, Error>)
+  {true}
+
+  method CreateAwsKmsDiscoveryMultiKeyring ( config: InternalConfig,  input: CreateAwsKmsDiscoveryMultiKeyringInput )
+    returns (output: Result<IKeyring, Error>)
+  {
+    var grantTokens :- GetValidGrantTokens(input.grantTokens);
+
+    var clientSupplier: Types.IClientSupplier;
+
+    //= compliance/framework/aws-kms/aws-kms-multi-keyrings.txt#2.6
+    //# If a regional client supplier is not passed,
+    //# then a default MUST be created that takes a region string and
+    //# generates a default AWS SDK client for the given region.
+    if input.clientSupplier.None? {
+      clientSupplier :- CreateDefaultClientSupplier(config, Types.CreateDefaultClientSupplierInput());
+    } else {
+      clientSupplier := input.clientSupplier.value;
+    }
+    output := DiscoveryMultiKeyring(
+      input.regions,
+      input.discoveryFilter,
+      clientSupplier,
+      Option.Some(grantTokens)
+    );
+  }
+
+  predicate CreateAwsKmsMrkKeyringEnsuresPublicly(input: CreateAwsKmsMrkKeyringInput, output: Result<IKeyring, Error>)
+  {true}
+
+  method CreateAwsKmsMrkKeyring ( config: InternalConfig,  input: CreateAwsKmsMrkKeyringInput )
+    returns (output: Result<IKeyring, Error>)
+  {
+    var _ :- ValidateKmsKeyId(input.kmsKeyId);
+    var grantTokens :- GetValidGrantTokens(input.grantTokens);
+    var keyring := new AwsKmsMrkKeyring.AwsKmsMrkKeyring(input.kmsClient, input.kmsKeyId, grantTokens);
+    return Success(keyring);
+  }
+
+
+  predicate CreateAwsKmsMrkMultiKeyringEnsuresPublicly(input: CreateAwsKmsMrkMultiKeyringInput, output: Result<IKeyring, Error>)
+  {true}
+
+  method CreateAwsKmsMrkMultiKeyring ( config: InternalConfig,  input: CreateAwsKmsMrkMultiKeyringInput )
+    returns (output: Result<IKeyring, Error>)
+  {
+    var grantTokens :- GetValidGrantTokens(input.grantTokens);
+
+    var clientSupplier: Types.IClientSupplier;
+
+    //= compliance/framework/aws-kms/aws-kms-mrk-multi-keyrings.txt#2.5
+    //# If a regional client supplier is
+    //# not passed, then a default MUST be created that takes a region string
+    //# and generates a default AWS SDK client for the given region.
+    if input.clientSupplier.None? {
+      clientSupplier :- CreateDefaultClientSupplier(config, Types.CreateDefaultClientSupplierInput());
+    } else {
+      clientSupplier := input.clientSupplier.value;
+    }
+    output := MrkAwareStrictMultiKeyring(
+      input.generator,
+      input.kmsKeyIds,
+      clientSupplier,
+      Option.Some(grantTokens)
+    );
+  }
+
+  predicate CreateAwsKmsMrkDiscoveryKeyringEnsuresPublicly(input: CreateAwsKmsMrkDiscoveryKeyringInput, output: Result<IKeyring, Error>)
+  {true}
+
+  method CreateAwsKmsMrkDiscoveryKeyring ( config: InternalConfig,  input: CreateAwsKmsMrkDiscoveryKeyringInput )
+    returns (output: Result<IKeyring, Error>)
+  {
+    if input.discoveryFilter.Some? {
+      var _ :- ValidateDiscoveryFilter(input.discoveryFilter.value);
+    }
+
+    //= compliance/framework/aws-kms/aws-kms-mrk-discovery-keyring.txt#2.6
+    //= type=implication
+    //# The keyring SHOULD fail initialization if the
+    //# provided region does not match the region of the KMS client.
+    var regionMatch := AwsKmsUtils.RegionMatch(input.kmsClient, input.region);
+    :- Need(regionMatch != Some(false),
+      Types.AwsCryptographicMaterialProvidersException(
+        message := "Provided client and region do not match"));
+
+    var grantTokens :- GetValidGrantTokens(input.grantTokens);
+    var keyring := new AwsKmsMrkDiscoveryKeyring.AwsKmsMrkDiscoveryKeyring(input.kmsClient, input.region, input.discoveryFilter, grantTokens);
+    return Success(keyring);
+  }
+
+
+  predicate CreateAwsKmsMrkDiscoveryMultiKeyringEnsuresPublicly(input: CreateAwsKmsMrkDiscoveryMultiKeyringInput, output: Result<IKeyring, Error>)
+  {true}
+
+  method CreateAwsKmsMrkDiscoveryMultiKeyring ( config: InternalConfig,  input: CreateAwsKmsMrkDiscoveryMultiKeyringInput )
+    returns (output: Result<IKeyring, Error>)
+  {
+    var grantTokens :- GetValidGrantTokens(input.grantTokens);
+
+    var clientSupplier: Types.IClientSupplier;
+
+    //= compliance/framework/aws-kms/aws-kms-mrk-multi-keyrings.txt#2.6
+    //# If a regional client supplier is not passed,
+    //# then a default MUST be created that takes a region string and
+    //# generates a default AWS SDK client for the given region.
+    if input.clientSupplier.None? {
+      clientSupplier :- CreateDefaultClientSupplier(config, Types.CreateDefaultClientSupplierInput());
+    } else {
+      clientSupplier := input.clientSupplier.value;
+    }
+    output := MrkAwareDiscoveryMultiKeyring(
+      input.regions,
+      input.discoveryFilter,
+      clientSupplier,
+      Option.Some(grantTokens)
+    );
+  }
+
+  predicate CreateMultiKeyringEnsuresPublicly(input: CreateMultiKeyringInput, output: Result<IKeyring, Error>)
+  {true}
+
+  method CreateMultiKeyring ( config: InternalConfig,  input: CreateMultiKeyringInput )
+    returns (output: Result<IKeyring, Error>)
+  {
+    :- Need(input.generator.Some? || |input.childKeyrings| > 0,
+      Types.AwsCryptographicMaterialProvidersException(
+        message := "Must include a generator keyring and/or at least one child keyring"));
+
+    var keyring := new MultiKeyring.MultiKeyring(input.generator, input.childKeyrings);
+    return Success(keyring);
+  }
+
+
+  predicate CreateRawAesKeyringEnsuresPublicly(input: CreateRawAesKeyringInput, output: Result<IKeyring, Error>)
+  {
+    //= compliance/framework/raw-aes-keyring.txt#2.1.1
+    //= type=implication
+    //# -  Raw AES keyring MUST NOT accept a key namespace of "aws-kms".
+      input.keyNamespace == "aws-kms"
+    ==>
+      output.Failure?
+  }
+
+  method CreateRawAesKeyring ( config: InternalConfig,  input: CreateRawAesKeyringInput )
+    returns (output: Result<IKeyring, Error>)
+  {
+    :- Need(input.keyNamespace != "aws-kms",
+      Types.AwsCryptographicMaterialProvidersException(
+        message := "keyNamespace must not be `aws-kms`"));
+
+    var wrappingAlg:Crypto.AES_GCM := match input.wrappingAlg
+      case ALG_AES128_GCM_IV12_TAG16 => Crypto.AES_GCM(
+          keyLength := 16,
+          tagLength := 16,
+          ivLength := 12
+        )
+      case ALG_AES192_GCM_IV12_TAG16 => Crypto.AES_GCM(
+          keyLength := 24,
+          tagLength := 16,
+          ivLength := 12
+        )
+      case ALG_AES256_GCM_IV12_TAG16 => Crypto.AES_GCM(
+          keyLength := 32,
+          tagLength := 16,
+          ivLength := 12
+        );
+
+    var namespaceAndName :- ParseKeyNamespaceAndName(input.keyNamespace, input.keyName);
+    var (namespace, name) := namespaceAndName;
+
+    :- Need(|input.wrappingKey| == 16 || |input.wrappingKey| == 24 || |input.wrappingKey| == 32,
+      Types.AwsCryptographicMaterialProvidersException(
+        message := "Invalid wrapping key length"));
+    :- Need(|input.wrappingKey| == wrappingAlg.keyLength as int,
+      Types.AwsCryptographicMaterialProvidersException(
+        message := "Wrapping key length does not match specified wrapping algorithm"));
+
+    var keyring := new RawAESKeyring
+      .RawAESKeyring(
+        namespace := namespace,
+        name := name,
+        key := input.wrappingKey,
+        wrappingAlgorithm := wrappingAlg,
+        cryptoPrimitives := config.crypto
+      );
+    return Success(keyring);
+  }
+
+
+  predicate CreateRawRsaKeyringEnsuresPublicly(input: CreateRawRsaKeyringInput, output: Result<IKeyring, Error>)
+  {
+    //= compliance/framework/raw-rsa-keyring.txt#2.1.1
+    //= type=implication
+    //# -  Raw RSA keyring MUST NOT accept a key namespace of "aws-kms".
+    && (input.keyNamespace == "aws-kms"
+    ==>
+      output.Failure?)
+    && (input.publicKey.None? && input.privateKey.None?
+      ==>
+        output.Failure?)
+  }
+
+  method CreateRawRsaKeyring ( config: InternalConfig,  input: CreateRawRsaKeyringInput )
+    returns (output: Result<IKeyring, Error>)
+  {
+    :- Need(input.keyNamespace != "aws-kms",
+        Types.AwsCryptographicMaterialProvidersException(
+      message := "keyNamespace must not be `aws-kms`"));
+    :- Need(input.publicKey.Some? || input.privateKey.Some?,
+        Types.AwsCryptographicMaterialProvidersException(
+      message := "A publicKey or a privateKey is required"));
+
+    var padding: Crypto.RSAPaddingMode := match input.paddingScheme
+      case PKCS1 => Crypto.RSAPaddingMode.PKCS1
+      case OAEP_SHA1_MGF1 => Crypto.RSAPaddingMode.OAEP_SHA1
+      case OAEP_SHA256_MGF1 => Crypto.RSAPaddingMode.OAEP_SHA256
+      case OAEP_SHA384_MGF1 => Crypto.RSAPaddingMode.OAEP_SHA384
+      case OAEP_SHA512_MGF1 => Crypto.RSAPaddingMode.OAEP_SHA512
+    ;
+
+    var namespaceAndName :- ParseKeyNamespaceAndName(input.keyNamespace, input.keyName);
+    var (namespace, name) := namespaceAndName;
+
+    var keyring := new RawRSAKeyring.RawRSAKeyring(
+      namespace := namespace,
+      name := name,
+      publicKey := input.publicKey,
+      privateKey := input.privateKey,
+      paddingScheme := padding,
+      cryptoPrimitives := config.crypto
+    );
+    return Success(keyring);
+  }
+ 
+
+  predicate CreateDefaultCryptographicMaterialsManagerEnsuresPublicly(input: CreateDefaultCryptographicMaterialsManagerInput, output: Result<ICryptographicMaterialsManager, Error>)
+  {true}
+
+  method CreateDefaultCryptographicMaterialsManager(config: InternalConfig, input: CreateDefaultCryptographicMaterialsManagerInput)
+    returns (output: Result<ICryptographicMaterialsManager, Error>)
+  {
+    var cmm := new DefaultCMM.OfKeyring(input.keyring, config.crypto);
+    return Success(cmm);
+  }
+
+  predicate CreateDefaultClientSupplierEnsuresPublicly(input: CreateDefaultClientSupplierInput, output: Result<IClientSupplier, Error>)
+  {true}
+
+  method CreateDefaultClientSupplier ( config: InternalConfig,  input: CreateDefaultClientSupplierInput )
+    returns (output: Result<IClientSupplier, Error>)
+  {
+    var clientSupplier := new DefaultClientSupplier.DefaultClientSupplier();
+    return Success(clientSupplier);
+  }
+
+  function method InitializeEncryptionMaterials ( config: InternalConfig,  input: InitializeEncryptionMaterialsInput )
+  : (output: Result<EncryptionMaterials, Error>)
+  {
+    Materials.InitializeEncryptionMaterials(input)
+  }
+
+  function method InitializeDecryptionMaterials ( config: InternalConfig,  input: InitializeDecryptionMaterialsInput )
+  : (output: Result<DecryptionMaterials, Error>)
+  {
+    Materials.InitializeDecryptionMaterials(input)
+  }
+
+  function method ValidEncryptionMaterialsTransition ( config: InternalConfig,  input: ValidEncryptionMaterialsTransitionInput )
+  : (output: Result<(), Error>)
+  {
+    :- Need(
+      Materials.ValidEncryptionMaterialsTransition(input.start, input.stop),
+      InvalidEncryptionMaterialsTransition( message := "Invalid Encryption Materials Transition" )
+    );
+    
+    Success(())
+  }
+
+  function method ValidDecryptionMaterialsTransition ( config: InternalConfig,  input: ValidDecryptionMaterialsTransitionInput )
+  : (output: Result<(), Error>)
+  {
+    :- Need(
+      Materials.DecryptionMaterialsTransitionIsValid(input.start, input.stop),
+      InvalidDecryptionMaterialsTransition( message := "Invalid Decryption Materials Transition")
+    );
+
+    Success(())
+  }
+
+  function method EncryptionMaterialsHasPlaintextDataKey ( config: InternalConfig,  input: EncryptionMaterials )
+    : (output: Result<(), Error>)
+  {
+    :- Need(
+      Materials.EncryptionMaterialsHasPlaintextDataKey(input),
+      InvalidDecryptionMaterials( message := "Invalid Encryption Materials")
+    );
+
+    Success(())
+  }
+  function method DecryptionMaterialsWithPlaintextDataKey ( config: InternalConfig,  input: DecryptionMaterials )
+    : (output: Result<(), Error>)
+  {
+    :- Need(
+      Materials.DecryptionMaterialsWithPlaintextDataKey(input),
+      InvalidDecryptionMaterials( message := "Invalid Decryption Materials")
+    );
+
+    Success(())
+  }
+
+  function method GetAlgorithmSuiteInfo ( config: InternalConfig,  input: seq<uint8> )
+  : (output: Result<AlgorithmSuiteInfo, Error>)
+  {
+    AlgorithmSuites.GetAlgorithmSuiteInfo(input)
+  }
+
+  function method ValidAlgorithmSuiteInfo ( config: InternalConfig,  input: AlgorithmSuiteInfo )
+  : (output: Result<(), Error>)
+  {
+    :- Need(AlgorithmSuites.AlgorithmSuite?(input),
+      InvalidAlgorithmSuiteInfo( message := "Invalid AlgorithmSuiteInfo" )
+    );
+
+    Success(())
+  }
+
+  function method ValidateCommitmentPolicyOnEncrypt ( config: InternalConfig,  input: ValidateCommitmentPolicyOnEncryptInput )
+  : (output: Result<(), Error>)
+  {
+    :- Commitment.ValidateCommitmentPolicyOnEncrypt(input.algorithm, input.commitmentPolicy);
+
+    Success(())
+  }
+
+  function method ValidateCommitmentPolicyOnDecrypt ( config: InternalConfig,  input: ValidateCommitmentPolicyOnDecryptInput )
+  : (output: Result<(), Error>)
+  {
+    :- Commitment.ValidateCommitmentPolicyOnDecrypt(input.algorithm, input.commitmentPolicy);
+
+    Success(())
+  }
+
+}
