AwsCryptographicMaterialProviders/src/CMMs/DefaultCMM.dfy
@@ -1,0 +1,271 @@
+// Copyright Amazon.com Inc. or its affiliates. All Rights Reserved.
+// SPDX-License-Identifier: Apache-2.0
+
+include "../../../src/StandardLibrary/Base64.dfy"
+include "../Materials.dfy"
+include "../AlgorithmSuites.dfy"
+include "../CMM.dfy"
+include "../Defaults.dfy"
+include "../Commitment.dfy"
+include "../../Model/AwsCryptographyMaterialProvidersTypes.dfy"
+
+module DefaultCMM {
+  import opened Wrappers
+  import opened UInt = StandardLibrary.UInt
+  import AlgorithmSuites
+  import Materials
+  import CMM
+  import Signature
+  import Base64
+  import UTF8
+  import Types = AwsCryptographyMaterialProvidersTypes
+  import Crypto = AwsCryptographyPrimitivesTypes
+  import Aws.Cryptography.Primitives
+  import Defaults
+  import Commitment
+
+  class DefaultCMM
+    extends CMM.VerifiableInterface
+  {
+    const cryptoPrimitives: Primitives.AtomicPrimitivesClient
+
+    predicate ValidState()
+    ensures ValidState() ==> History in Modifies
+    {
+      && History in Modifies
+      && keyring.ValidState()
+      && cryptoPrimitives.ValidState()
+      && keyring.Modifies <= Modifies
+      && cryptoPrimitives.Modifies <= Modifies
+      && History !in keyring.Modifies
+      && History !in cryptoPrimitives.Modifies
+    }
+
+    const keyring: Types.IKeyring
+
+    constructor OfKeyring(
+      k: Types.IKeyring,
+      c: Primitives.AtomicPrimitivesClient
+    )
+      requires k.ValidState() && c.ValidState()
+      ensures keyring == k && cryptoPrimitives == c
+      ensures
+        && ValidState()
+        && fresh(this)
+        && fresh(History)
+        && fresh(Modifies - cryptoPrimitives.Modifies - keyring.Modifies)
+      ensures Modifies == { History } + keyring.Modifies + cryptoPrimitives.Modifies
+    {
+      keyring := k;
+      cryptoPrimitives := c;
+
+      History := new Types.ICryptographicMaterialsManagerCallHistory();
+      Modifies := { History } + c.Modifies + k.Modifies;
+    }
+
+    predicate GetEncryptionMaterialsEnsuresPublicly(input: Types.GetEncryptionMaterialsInput, output: Result<Types.GetEncryptionMaterialsOutput, Types.Error>)
+    {true}
+
+    method GetEncryptionMaterials'(
+      input: Types.GetEncryptionMaterialsInput
+    )
+      returns (output: Result<Types.GetEncryptionMaterialsOutput, Types.Error>)
+      requires
+      && ValidState() 
+      modifies Modifies - {History}
+      // Dafny will skip type parameters when generating a default decreases clause.
+      decreases Modifies - {History}
+      ensures
+      && ValidState()
+      ensures GetEncryptionMaterialsEnsuresPublicly(input, output)
+      ensures unchanged(History)
+      ensures output.Success?
+      ==>
+        && Materials.EncryptionMaterialsHasPlaintextDataKey(output.value.encryptionMaterials)
+        && (
+          output.value.encryptionMaterials.algorithmSuite.signature.ECDSA?
+        <==>
+          Materials.EC_PUBLIC_KEY_FIELD in output.value.encryptionMaterials.encryptionContext
+        )
+      ensures Materials.EC_PUBLIC_KEY_FIELD in input.encryptionContext ==> output.Failure?
+
+      // Make sure that we returned the correct algorithm suite, either as specified in
+      // the input or, if that was not given, the default for the provided commitment policy
+      ensures
+        && output.Success?
+      ==>
+        (if input.algorithmSuiteId.Some? then
+          //= compliance/framework/default-cmm.txt#2.6.1
+          //= type=implication
+          //# *  If the encryption materials request (cmm-interface.md#encryption-
+          //# materials-request) does contain an algorithm suite, the encryption
+          //# materials returned MUST contain the same algorithm suite.
+          output.value.encryptionMaterials.algorithmSuite.id == input.algorithmSuiteId.value
+        else
+            //= compliance/framework/default-cmm.txt#2.6.1
+            //= type=implication
+            //# *  If the encryption materials request (cmm-interface.md#encryption-
+            //# materials-request) does not contain an algorithm suite, the
+            //# operation MUST add the default algorithm suite for the commitment
+            //# policy (../client-apis/client.md#commitment-policy) as the
+            //# algorithm suite in the encryption materials returned.
+            //
+            //= compliance/client-apis/client.txt#2.4.2.1
+            //= type=implication
+            //# *  "03 78" MUST be the default algorithm suite
+            //
+            //= compliance/client-apis/client.txt#2.4.2.2
+            //= type=implication
+            //# *  "05 78" MUST be the default algorithm suite
+            //
+            //= compliance/client-apis/client.txt#2.4.2.3
+            //= type=implication
+            //# *  "05 78" MUST be the default algorithm suite
+            && input.algorithmSuiteId.None?
+            && output.value.encryptionMaterials.algorithmSuite.id
+              == Defaults.GetAlgorithmSuiteForCommitmentPolicy(input.commitmentPolicy))
+
+      //= compliance/framework/default-cmm.txt#2.6.1
+      //= type=implication
+      //# *  If the encryption materials request (cmm-interface.md#encryption-
+      //# materials-request) does contain an algorithm suite, the request
+      //# MUST fail if the algorithm suite is not supported by the
+      //# commitment policy (../client-apis/client.md#commitment-policy) on
+      //# the request.
+      ensures
+        && input.algorithmSuiteId.Some?
+        && Commitment.ValidateCommitmentPolicyOnEncrypt(input.algorithmSuiteId.value, input.commitmentPolicy).Fail?
+      ==>
+        output.Failure?
+    {
+      :- Need(Materials.EC_PUBLIC_KEY_FIELD !in input.encryptionContext,
+        Types.AwsCryptographicMaterialProvidersException(
+          message :="Reserved Field found in EncryptionContext keys."));
+
+      var algorithmId := if input.algorithmSuiteId.Some? then
+        input.algorithmSuiteId.value
+      else
+        Defaults.GetAlgorithmSuiteForCommitmentPolicy(input.commitmentPolicy);
+
+      :- Commitment.ValidateCommitmentPolicyOnEncrypt(
+        algorithmId, input.commitmentPolicy
+      );
+
+      var suite := AlgorithmSuites.GetSuite(algorithmId);
+      var signingKey: Option<seq<uint8>>;
+      var verificationKey: Option<seq<uint8>>;
+      if suite.signature.ECDSA? {
+        var maybeECDSAPair := cryptoPrimitives.GenerateECDSASignatureKey(
+          Crypto.GenerateECDSASignatureKeyInput(
+            signatureAlgorithm := suite.signature.ECDSA.curve
+          )
+        );
+        var pair :- maybeECDSAPair.MapFailure(e => Types.AwsCryptographyPrimitives(e));
+        signingKey := Some(pair.signingKey);
+        verificationKey := Some(pair.verificationKey);
+      } else {
+        assert  suite.signature.None?;
+        signingKey := None;
+        verificationKey := None;
+      }
+
+      var materials :- Materials.InitializeEncryptionMaterials(
+        Types.InitializeEncryptionMaterialsInput(
+          algorithmSuiteId := algorithmId,
+          encryptionContext := input.encryptionContext,
+          signingKey := signingKey,
+          verificationKey := verificationKey
+        )
+      );
+
+      var result :- keyring.OnEncrypt(Types.OnEncryptInput(materials:=materials));
+      var encryptionMaterialsOutput := Types.GetEncryptionMaterialsOutput(encryptionMaterials:=result.materials);
+
+      :- Need(
+        Materials.EncryptionMaterialsHasPlaintextDataKey(encryptionMaterialsOutput.encryptionMaterials),
+        Types.AwsCryptographicMaterialProvidersException(
+          message := "Could not retrieve materials required for encryption"));
+
+      // For Dafny keyrings this is a trivial statement
+      // because they implement a trait that ensures this.
+      // However not all keyrings are Dafny keyrings.
+      // Customers can create custom keyrings.
+      :- Need(
+        Materials.ValidEncryptionMaterialsTransition(materials, encryptionMaterialsOutput.encryptionMaterials),
+        Types.AwsCryptographicMaterialProvidersException(
+          message := "Keyring returned an invalid response"));
+
+      output := Success(encryptionMaterialsOutput);
+    }
+
+    predicate DecryptMaterialsEnsuresPublicly(input: Types.DecryptMaterialsInput, output: Result<Types.DecryptMaterialsOutput, Types.Error>)
+    {true}
+
+    method DecryptMaterials'(
+      input: Types.DecryptMaterialsInput
+    )
+      returns (output: Result<Types.DecryptMaterialsOutput, Types.Error>)
+      requires
+      && ValidState() 
+      modifies Modifies - {History}
+      // Dafny will skip type parameters when generating a default decreases clause.
+      decreases Modifies - {History}
+      ensures
+      && ValidState()
+      ensures DecryptMaterialsEnsuresPublicly(input, output)
+      ensures unchanged(History)
+      ensures output.Success?
+      ==>
+        && Materials.DecryptionMaterialsWithPlaintextDataKey(output.value.decryptionMaterials)
+
+      // If the input has either
+      //   (a) an unsigned algorithm suite and the aws-crypto-public-key encryption context key
+      //   (b) a signing algorithm suite and no aws-crypto-public-key encryption context key
+      // then the operation SHOULD fail.
+      // (Here we strengthen the SHOULD to a MUST.)
+      ensures
+        (
+          AlgorithmSuites.GetSuite(input.algorithmSuiteId).signature.None?
+          <==>
+          (Materials.EC_PUBLIC_KEY_FIELD in input.encryptionContext)
+        )
+        ==> output.Failure?
+
+      //= compliance/framework/default-cmm.txt#2.6.2
+      //= type=implication
+      //# The request MUST fail if the algorithm suite on the request is not
+      //# supported by the commitment policy (../client-apis/
+      //# client.md#commitment-policy) on the request.
+      ensures Commitment.ValidateCommitmentPolicyOnDecrypt(input.algorithmSuiteId, input.commitmentPolicy).Fail?
+      ==>
+        output.Failure?
+    {
+      :- Commitment.ValidateCommitmentPolicyOnDecrypt(
+        input.algorithmSuiteId, input.commitmentPolicy
+      );
+
+      var materials :- Materials.InitializeDecryptionMaterials(
+        Types.InitializeDecryptionMaterialsInput(
+          algorithmSuiteId := input.algorithmSuiteId,
+          encryptionContext := input.encryptionContext
+        )
+      );
+
+      var result :- keyring.OnDecrypt(Types.OnDecryptInput(
+        materials:=materials,
+        encryptedDataKeys:=input.encryptedDataKeys
+      ));
+
+      // For Dafny keyrings this is a trivial statement
+      // because they implement a trait that ensures this.
+      // However not all keyrings are Dafny keyrings.
+      // Customers can create custom keyrings.
+      :- Need(
+        Materials.DecryptionMaterialsTransitionIsValid(materials, result.materials),
+        Types.AwsCryptographicMaterialProvidersException(
+          message := "Keyring.OnDecrypt failed to decrypt the plaintext data key."));
+
+      return Success(Types.DecryptMaterialsOutput(decryptionMaterials:=result.materials));
+    }
+  }
+}
