AwsCryptographicMaterialProviders/src/Defaults.dfy
@@ -1,0 +1,31 @@
+// Copyright Amazon.com Inc. or its affiliates. All Rights Reserved.
+// SPDX-License-Identifier: Apache-2.0
+
+include "../Model/AwsCryptographyMaterialProvidersTypes.dfy"
+
+module Defaults {
+  import opened AwsCryptographyMaterialProvidersTypes
+
+  /* Returns the default algorithm suite for the given commitment policy */
+  function method GetAlgorithmSuiteForCommitmentPolicy(commitmentPolicy:CommitmentPolicy):
+    (output: AlgorithmSuiteId)
+
+    ensures
+      commitmentPolicy == CommitmentPolicy.ESDK(FORBID_ENCRYPT_ALLOW_DECRYPT)
+      ==>
+      output == AlgorithmSuiteId.ESDK(ALG_AES_256_GCM_IV12_TAG16_HKDF_SHA384_ECDSA_P384)
+
+    ensures
+      || commitmentPolicy == CommitmentPolicy.ESDK(REQUIRE_ENCRYPT_ALLOW_DECRYPT)
+      || commitmentPolicy == CommitmentPolicy.ESDK(REQUIRE_ENCRYPT_REQUIRE_DECRYPT)
+      ==>
+      output == AlgorithmSuiteId.ESDK(ALG_AES_256_GCM_HKDF_SHA512_COMMIT_KEY_ECDSA_P384)
+  {
+    match commitmentPolicy
+      case ESDK(c) => (
+        match c
+          case FORBID_ENCRYPT_ALLOW_DECRYPT() => AlgorithmSuiteId.ESDK(ALG_AES_256_GCM_IV12_TAG16_HKDF_SHA384_ECDSA_P384)
+          case _ => AlgorithmSuiteId.ESDK(ALG_AES_256_GCM_HKDF_SHA512_COMMIT_KEY_ECDSA_P384)
+      )
+  }
+}
