AwsCryptographicMaterialProviders/src/Index.dfy
@@ -1,0 +1,46 @@
+// Copyright Amazon.com Inc. or its affiliates. All Rights Reserved.
+// SPDX-License-Identifier: Apache-2.0
+
+include "AwsCryptographyMaterialProvidersOperations.dfy"
+
+module
+  {:extern "Dafny.Aws.Cryptography.MaterialProviders" }
+  MaterialProviders refines AbstractAwsCryptographyMaterialProvidersService
+{
+
+  import Operations = AwsCryptographyMaterialProvidersOperations
+  import Aws.Cryptography.Primitives
+
+  function method DefaultMaterialProvidersConfig(): MaterialProvidersConfig
+  {
+    MaterialProvidersConfig
+  }
+
+  method MaterialProviders(config: MaterialProvidersConfig)
+    returns (res: Result<MaterialProvidersClient, Error>)
+  {
+    var maybeCrypto := Primitives.AtomicPrimitives();
+    var crypto :- maybeCrypto
+      .MapFailure(e => AwsCryptographyPrimitives(e));
+    var client := new MaterialProvidersClient(Operations.Config( crypto := crypto ));
+    return Success(client);
+  }
+
+  class MaterialProvidersClient... {
+
+    predicate ValidState()
+    {
+      && Operations.ValidInternalConfig?(config)
+      && Modifies == Operations.ModifiesInternalConfig(config) + {History}
+    }
+
+    constructor(config: Operations.InternalConfig)
+    {
+      this.config := config;
+      History := new IAwsCryptographicMaterialProvidersClientCallHistory();
+      Modifies := Operations.ModifiesInternalConfig(config) + {History};
+    }
+
+  }
+
+}
