AwsCryptographicMaterialProviders/src/Keyrings/AwsKms/AwsKmsMrkKeyring.dfy
@@ -1,0 +1,680 @@
+// Copyright Amazon.com Inc. or its affiliates. All Rights Reserved.
+// SPDX-License-Identifier: Apache-2.0
+
+include "../../../../libraries/src/Collections/Sequences/Seq.dfy"
+
+include "../../../../src/StandardLibrary/Actions.dfy"
+include "../../../Model/AwsCryptographyMaterialProvidersTypes.dfy"
+
+include "Constants.dfy"
+include "AwsKmsMrkMatchForDecrypt.dfy"
+include "AwsKmsArnParsing.dfy"
+include "AwsKmsUtils.dfy"
+include "../../Keyring.dfy"
+include "../../Materials.dfy"
+include "../../AlgorithmSuites.dfy"
+
+module AwsKmsMrkKeyring {
+  import opened StandardLibrary
+  import opened Wrappers
+  import opened UInt = StandardLibrary.UInt
+  import opened AwsKmsArnParsing
+  import opened AwsKmsUtils
+  import Types = AwsCryptographyMaterialProvidersTypes
+  import KMS = Types.ComAmazonawsKmsTypes
+  import opened Seq
+  import opened Actions
+  import opened Constants
+  import opened A = AwsKmsMrkMatchForDecrypt
+  import Keyring
+  import Materials
+  import AlgorithmSuites
+  import UTF8
+
+  //= compliance/framework/aws-kms/aws-kms-mrk-keyring.txt#2.5
+  //= type=implication
+  //# MUST implement the AWS Encryption SDK Keyring interface (../keyring-
+  //# interface.md#interface)
+  class AwsKmsMrkKeyring
+    extends Keyring.VerifiableInterface
+  {
+
+    const client: KMS.IKeyManagementServiceClient
+    const awsKmsKey: AwsKmsIdentifierString
+    const awsKmsArn: AwsKmsIdentifier
+    const grantTokens: KMS.GrantTokenList
+
+    predicate ValidState()
+    ensures ValidState() ==> History in Modifies
+    {
+      && History in Modifies
+      && client.ValidState()
+      && client.Modifies <= Modifies
+      && History !in client.Modifies
+    }
+
+    constructor (
+      //= compliance/framework/aws-kms/aws-kms-mrk-keyring.txt#2.6
+      //= type=implication
+      //# The AWS KMS SDK client MUST NOT be null.
+      client: KMS.IKeyManagementServiceClient,
+      awsKmsKey: string,
+      grantTokens: KMS.GrantTokenList
+    )
+      //= compliance/framework/aws-kms/aws-kms-mrk-keyring.txt#2.6
+      //= type=implication
+      //# The AWS KMS key identifier MUST NOT be null or empty.
+      //# The AWS KMS
+      //# key identifier MUST be a valid identifier (aws-kms-key-arn.md#a-
+      //# valid-aws-kms-identifier).
+      requires ParseAwsKmsIdentifier(awsKmsKey).Success?
+      requires UTF8.IsASCIIString(awsKmsKey)
+      requires 0 < |awsKmsKey| <= MAX_AWS_KMS_IDENTIFIER_LENGTH
+      requires client.ValidState()
+      ensures
+        && this.client      == client
+        && this.awsKmsKey   == awsKmsKey
+        && this.grantTokens == grantTokens
+      ensures ValidState() && fresh(this) && fresh(History) && fresh(Modifies - client.Modifies)
+    {
+      var parsedAwsKmsId  := ParseAwsKmsIdentifier(awsKmsKey);
+      this.client         := client;
+      this.awsKmsKey      := awsKmsKey;
+      this.awsKmsArn      := parsedAwsKmsId.value;
+      this.grantTokens    := grantTokens;
+
+      History := new Types.IKeyringCallHistory();
+      Modifies := {History} + client.Modifies;
+    }
+
+    predicate OnEncryptEnsuresPublicly ( input: Types.OnEncryptInput , output: Result<Types.OnEncryptOutput, Types.Error> ) {true}
+
+    //= compliance/framework/aws-kms/aws-kms-mrk-keyring.txt#2.7
+    //= type=implication
+    //# OnEncrypt MUST take encryption materials (../structures.md#encryption-
+    //# materials) as input.
+    method {:vcs_split_on_every_assert} OnEncrypt'(input: Types.OnEncryptInput)
+      returns (output: Result<Types.OnEncryptOutput, Types.Error>)
+      requires ValidState()
+      modifies Modifies - {History}
+      decreases Modifies - {History}
+      ensures ValidState()
+      ensures unchanged(History)
+      ensures OnEncryptEnsuresPublicly(input, output)
+      ensures output.Success?
+      ==>
+        && Materials.ValidEncryptionMaterialsTransition(
+          input.materials,
+          output.value.materials
+        )
+        && StringifyEncryptionContext(input.materials.encryptionContext).Success?
+
+      //= compliance/framework/aws-kms/aws-kms-mrk-keyring.txt#2.7
+      //= type=implication
+      //# If the input encryption materials (../structures.md#encryption-
+      //# materials) do not contain a plaintext data key OnEncrypt MUST attempt
+      //# to generate a new plaintext data key by calling AWS KMS
+      //# GenerateDataKey (https://docs.aws.amazon.com/kms/latest/APIReference/
+      //# API_GenerateDataKey.html).
+      ensures
+        && input.materials.plaintextDataKey.None?
+        && StringifyEncryptionContext(input.materials.encryptionContext).Success?
+      ==>
+        0 < |client.History.GenerateDataKey|
+
+      ensures
+        var maybeStringifiedEncCtx := StringifyEncryptionContext(input.materials.encryptionContext);
+        && input.materials.plaintextDataKey.None?
+        && KMS.IsValid_KeyIdType(awsKmsKey)
+        && maybeStringifiedEncCtx.Success?
+      ==> (
+          //= compliance/framework/aws-kms/aws-kms-mrk-keyring.txt#2.7
+          //= type=implication
+          //# The keyring MUST call
+          //# AWS KMS GenerateDataKeys with a request constructed as follows:
+          && var GenerateDataKeyRequest := KMS.GenerateDataKeyRequest(
+            KeyId := awsKmsKey,
+            EncryptionContext := Option.Some(maybeStringifiedEncCtx.Extract()),
+            GrantTokens := Option.Some(grantTokens),
+            NumberOfBytes := Option.Some(AlgorithmSuites.GetEncryptKeyLength(input.materials.algorithmSuite)),
+            KeySpec := Option.None
+          );
+        //= compliance/framework/aws-kms/aws-kms-mrk-keyring.txt#2.7
+        //= type=implication
+        //# If the keyring calls AWS KMS GenerateDataKeys, it MUST use the
+        //# configured AWS KMS client to make the call.
+        && GenerateDataKeyRequest == Last(client.History.GenerateDataKey).input
+      )
+
+      //= compliance/framework/aws-kms/aws-kms-mrk-keyring.txt#2.7
+      //= type=implication
+      //# *  OnEncrypt MUST output the modified encryption materials
+      //# (../structures.md#encryption-materials)
+      ensures
+        && input.materials.plaintextDataKey.None?
+        && output.Success?
+      ==>
+        && Last(client.History.GenerateDataKey).output.Success?
+        && output.value.materials.plaintextDataKey.Some?
+        && |output.value.materials.encryptedDataKeys| == |input.materials.encryptedDataKeys| + 1
+        && var suite := input.materials.algorithmSuite;
+        && var GenerateDataKeyResponse := Last(client.History.GenerateDataKey).output.value;
+        && GenerateDataKeyResponse.Plaintext.Some?
+        && GenerateDataKeyResponse.CiphertextBlob.Some?
+        && GenerateDataKeyResponse.KeyId.Some?
+        && UTF8.Encode(GenerateDataKeyResponse.KeyId.value).Success?
+        //= compliance/framework/aws-kms/aws-kms-mrk-keyring.txt#2.7
+        //= type=implication
+        //# If the Generate Data Key call succeeds, OnEncrypt MUST verify that
+        //# the response "Plaintext" length matches the specification of the
+        //# algorithm suite (../algorithm-suites.md)'s Key Derivation Input Length
+        //# field.
+        && AlgorithmSuites.GetEncryptKeyLength(suite) as int == |GenerateDataKeyResponse.Plaintext.value|
+        //= compliance/framework/aws-kms/aws-kms-mrk-keyring.txt#2.7
+        //= type=implication
+        //# If verified, OnEncrypt MUST do the following with the response
+        //# from AWS KMS GenerateDataKey
+        //# (https://docs.aws.amazon.com/kms/latest/APIReference/
+        //# API_GenerateDataKey.html):
+        && Last(output.value.materials.encryptedDataKeys).ciphertext
+          == GenerateDataKeyResponse.CiphertextBlob.value
+        && output.value.materials.plaintextDataKey.value
+          == GenerateDataKeyResponse.Plaintext.value
+        && Last(output.value.materials.encryptedDataKeys).keyProviderInfo
+          == UTF8.Encode(GenerateDataKeyResponse.KeyId.value).value
+
+      //= compliance/framework/aws-kms/aws-kms-mrk-keyring.txt#2.7
+      //# If the call to AWS KMS GenerateDataKey
+      //# (https://docs.aws.amazon.com/kms/latest/APIReference/
+      //# API_GenerateDataKey.html) does not succeed, OnEncrypt MUST NOT modify
+      //# the encryption materials (../structures.md#encryption-materials) and
+      //# MUST fail.
+      ensures
+        && input.materials.plaintextDataKey.None?
+        && StringifyEncryptionContext(input.materials.encryptionContext).Success?
+        && |client.History.GenerateDataKey| == |old(client.History.GenerateDataKey)| + 1
+        && Last(client.History.GenerateDataKey).output.Failure?
+      ==>
+        output.Failure?
+
+      ensures
+        && input.materials.plaintextDataKey.Some?
+        && StringifyEncryptionContext(input.materials.encryptionContext).Success?
+        && KMS.IsValid_PlaintextType(input.materials.plaintextDataKey.value)
+      ==>
+        |client.History.Encrypt| == |old(client.History.Encrypt)| + 1
+
+      ensures
+        var maybeStringifiedEncCtx := StringifyEncryptionContext(input.materials.encryptionContext);
+        && input.materials.plaintextDataKey.Some?
+        && KMS.IsValid_PlaintextType(input.materials.plaintextDataKey.value)
+        && maybeStringifiedEncCtx.Success?
+      ==>
+        //= compliance/framework/aws-kms/aws-kms-mrk-keyring.txt#2.7
+        //= type=implication
+        //# The keyring MUST call AWS KMS Encrypt
+        //# (https://docs.aws.amazon.com/kms/latest/APIReference/
+        //# API_Encrypt.html) using the configured AWS KMS client.      
+        && |client.History.Encrypt| == |old(client.History.Encrypt)| + 1
+        //= compliance/framework/aws-kms/aws-kms-mrk-keyring.txt#2.7
+        //= type=implication
+        //# The keyring
+        //# MUST AWS KMS Encrypt call with a request constructed as follows:
+        && var EncryptRequest := KMS.EncryptRequest(
+          KeyId := awsKmsKey,
+          Plaintext := input.materials.plaintextDataKey.value,
+          EncryptionContext := Option.Some(maybeStringifiedEncCtx.Extract()),
+          GrantTokens := Option.Some(grantTokens),
+          EncryptionAlgorithm := Option.None
+        );
+        //= compliance/framework/aws-kms/aws-kms-mrk-keyring.txt#2.7
+        //= type=implication
+        //# If the input encryption materials (../structures.md#encryption-
+        //# materials) do contain a plaintext data key, OnEncrypt MUST attempt to
+        //# encrypt the plaintext data key using the configured AWS KMS key
+        //# identifier.
+        && EncryptRequest == Last(client.History.Encrypt).input
+
+      //= compliance/framework/aws-kms/aws-kms-mrk-keyring.txt#2.7
+      //= type=implication
+      //# If all Encrypt calls succeed, OnEncrypt MUST output the modified
+      //# encryption materials (../structures.md#encryption-materials).
+      ensures
+        && input.materials.plaintextDataKey.Some?
+        && KMS.IsValid_PlaintextType(input.materials.plaintextDataKey.value)
+        && output.Success?
+      ==>
+        && Last(client.History.Encrypt).output.Success?
+        && var EncryptResponse := Last(client.History.Encrypt).output.value;
+        && EncryptResponse.CiphertextBlob.Some?
+        && EncryptResponse.KeyId.Some?
+        && UTF8.Encode(EncryptResponse.KeyId.value).Success?
+        //= compliance/framework/aws-kms/aws-kms-mrk-keyring.txt#2.7
+        //= type=implication
+        //# If verified, OnEncrypt MUST do the following with the
+        //# response from AWS KMS Encrypt
+        //# (https://docs.aws.amazon.com/kms/latest/APIReference/
+        //# API_Encrypt.html):
+        && |output.value.materials.encryptedDataKeys| == |input.materials.encryptedDataKeys| + 1
+        && Last(output.value.materials.encryptedDataKeys).ciphertext
+          == EncryptResponse.CiphertextBlob.value
+        && Last(output.value.materials.encryptedDataKeys).keyProviderInfo
+          == UTF8.Encode(EncryptResponse.KeyId.value).value
+
+      //= compliance/framework/aws-kms/aws-kms-mrk-keyring.txt#2.7
+      //= type=implication
+      //# If the call to AWS KMS Encrypt
+      //# (https://docs.aws.amazon.com/kms/latest/APIReference/
+      //# API_Encrypt.html) does not succeed, OnEncrypt MUST fail.
+      ensures
+        && input.materials.plaintextDataKey.Some?
+        && StringifyEncryptionContext(input.materials.encryptionContext).Success?
+        && |client.History.Encrypt| == |old(client.History.Encrypt)| + 1
+        && Last(client.History.Encrypt).output.Failure?
+      ==>
+        output.Failure?
+    {
+
+      var materials := input.materials;
+      var suite := input.materials.algorithmSuite;
+      var stringifiedEncCtx :- StringifyEncryptionContext(input.materials.encryptionContext);
+      if materials.plaintextDataKey.None? {
+
+        var generatorRequest := KMS.GenerateDataKeyRequest(
+          KeyId := awsKmsKey,
+          EncryptionContext := Option.Some(stringifiedEncCtx),
+          GrantTokens := Option.Some(grantTokens),
+          NumberOfBytes := Option.Some(AlgorithmSuites.GetEncryptKeyLength(suite)),
+          KeySpec := Option.None
+        );
+
+        var maybeGenerateResponse := client.GenerateDataKey(generatorRequest);
+
+        var generateResponse :- maybeGenerateResponse
+          .MapFailure(e => Types.ComAmazonawsKms(ComAmazonawsKms := e));
+
+        //= compliance/framework/aws-kms/aws-kms-mrk-keyring.txt#2.7
+        //# The Generate Data Key response's "KeyId" MUST be A valid AWS
+        //# KMS key ARN (aws-kms-key-arn.md#identifying-an-aws-kms-
+        //# multi-region-key).
+        :- Need(
+          && generateResponse.KeyId.Some?
+          && ParseAwsKmsIdentifier(generateResponse.KeyId.value).Success?,
+          Types.AwsCryptographicMaterialProvidersException( message := "Invalid response from KMS GenerateDataKey: Invalid Key Id")
+        );
+        var keyId := generateResponse.KeyId.value;
+        var providerInfo :- UTF8.Encode(keyId).MapFailure(WrapStringToError);
+        :- Need(|providerInfo| < UINT16_LIMIT,
+          Types.AwsCryptographicMaterialProvidersException( message := "Invalid response from KMS GenerateDataKey: AWS KMS Key ID too long."));
+
+        :- Need(
+          && generateResponse.Plaintext.Some?
+          && AlgorithmSuites.GetEncryptKeyLength(suite) as nat == |generateResponse.Plaintext.value|,
+          Types.AwsCryptographicMaterialProvidersException( message := "Invalid response from KMS GenerateDataKey: Invalid data key")
+        );
+        var plaintextDataKey := generateResponse.Plaintext.value;
+
+        :- Need(
+          && generateResponse.CiphertextBlob.Some?
+          && KMS.IsValid_CiphertextType(generateResponse.CiphertextBlob.value),
+          Types.AwsCryptographicMaterialProvidersException( message := "Returned ciphertext is invalid length"));
+        var ciphertext :- assert generateResponse.CiphertextBlob;
+
+        var edk := Types.EncryptedDataKey(
+          keyProviderId := PROVIDER_ID,
+          keyProviderInfo := providerInfo,
+          ciphertext := ciphertext
+        );
+
+        var outputMaterials :- Materials.EncryptionMaterialAddDataKey(materials, plaintextDataKey, [edk]);
+        var result := Types.OnEncryptOutput(
+          materials := outputMaterials
+        );
+        return Success(result);
+      } else {
+        :- Need(KMS.IsValid_PlaintextType(materials.plaintextDataKey.value),
+          Types.AwsCryptographicMaterialProvidersException( message := "PlaintextDataKey is invalid length")
+        );
+        var encryptRequest := KMS.EncryptRequest(
+            KeyId := awsKmsKey,
+            Plaintext := materials.plaintextDataKey.value,
+            EncryptionContext := Option.Some(stringifiedEncCtx),
+            GrantTokens := Option.Some(grantTokens),
+            EncryptionAlgorithm := Option.None
+        );
+        var maybeEncryptResponse := client.Encrypt(encryptRequest);
+
+        var encryptResponse :- maybeEncryptResponse
+          .MapFailure(e => Types.ComAmazonawsKms(ComAmazonawsKms := e));
+
+        //= compliance/framework/aws-kms/aws-kms-mrk-keyring.txt#2.7
+        //# If the Encrypt call succeeds the response's "KeyId" MUST be A valid
+        //# AWS KMS key ARN (aws-kms-key-arn.md#a-valid-aws-kms-arn).
+        :- Need(
+          && encryptResponse.KeyId.Some?
+          && ParseAwsKmsIdentifier(encryptResponse.KeyId.value).Success?,
+          Types.AwsCryptographicMaterialProvidersException( message := "Invalid response from AWS KMS Encrypt: Invalid Key Id")
+        );
+
+        :- Need(encryptResponse.CiphertextBlob.Some?,
+          Types.AwsCryptographicMaterialProvidersException( message := "Invalid response from AWS KMS Encrypt: Invalid Ciphertext Blob")
+        );
+
+        var providerInfo :- UTF8
+          .Encode(encryptResponse.KeyId.Extract())
+          .MapFailure(WrapStringToError);
+        :- Need(|providerInfo| < UINT16_LIMIT,
+          Types.AwsCryptographicMaterialProvidersException( message := "AWS KMS Key ID too long."));
+
+        var edk := Types.EncryptedDataKey(
+          keyProviderId := PROVIDER_ID,
+          keyProviderInfo := providerInfo,
+          ciphertext := encryptResponse.CiphertextBlob.value
+        );
+
+        var outputMaterials :- Materials.EncryptionMaterialAddEncryptedDataKeys(materials, [edk]);
+        var result := Types.OnEncryptOutput(
+          materials := outputMaterials
+        );
+        return Success(result);
+      }
+    }
+
+    predicate OnDecryptEnsuresPublicly ( input: Types.OnDecryptInput , output: Result<Types.OnDecryptOutput, Types.Error> ) {true}
+
+    //= compliance/framework/aws-kms/aws-kms-mrk-keyring.txt#2.8
+    //= type=implication
+    //# OnDecrypt MUST take decryption materials (../structures.md#decryption-
+    //# materials) and a list of encrypted data keys
+    //# (../structures.md#encrypted-data-key) as input.
+    method OnDecrypt'(
+      input: Types.OnDecryptInput
+    )
+      returns (output: Result<Types.OnDecryptOutput, Types.Error>)
+      requires ValidState()
+      modifies Modifies - {History}
+      decreases Modifies - {History}
+      ensures ValidState()
+      ensures unchanged(History)
+      ensures OnDecryptEnsuresPublicly(input, output)
+      ensures output.Success?
+      ==>
+        && Materials.DecryptionMaterialsTransitionIsValid(
+          input.materials,
+          output.value.materials
+        )
+
+      ensures
+        && input.materials.plaintextDataKey.None?
+        && output.Success?
+      ==>
+        && output.value.materials.plaintextDataKey.Some?
+        && var maybeStringifiedEncCtx := StringifyEncryptionContext(input.materials.encryptionContext);
+        && maybeStringifiedEncCtx.Success?
+        //= compliance/framework/aws-kms/aws-kms-mrk-keyring.txt#2.8
+        //= type=implication
+        //# * The length of the response's "Plaintext" MUST equal the key
+        //# derivation input length (../algorithm-suites.md#key-derivation-
+        //# input-length) specified by the algorithm suite (../algorithm-
+        //# suites.md) included in the input decryption materials
+        //# (../structures.md#decryption-materials).
+        && var suite := input.materials.algorithmSuite;
+        && AlgorithmSuites.GetEncryptKeyLength(suite) as nat == |output.value.materials.plaintextDataKey.value|
+        && 0 < |client.History.Decrypt|
+
+        && exists edk | edk in input.encryptedDataKeys
+        ::
+          //= compliance/framework/aws-kms/aws-kms-mrk-keyring.txt#2.8
+          //= type=implication
+          //# *  Its provider ID MUST exactly match the value "aws-kms".
+          && edk.keyProviderId == PROVIDER_ID
+          && KMS.IsValid_CiphertextType(edk.ciphertext)
+          && Last(client.History.Decrypt).output.Success?
+          && KMS.DecryptRequest(
+            KeyId := Option.Some(awsKmsKey),
+            CiphertextBlob :=  edk.ciphertext,
+            EncryptionContext := Option.Some(maybeStringifiedEncCtx.Extract()),
+            GrantTokens := Option.Some(grantTokens),
+            EncryptionAlgorithm := Option.None()
+          ) == Last(client.History.Decrypt).input
+          //= compliance/framework/aws-kms/aws-kms-mrk-keyring.txt#2.8
+          //= type=implication
+          //# To attempt to decrypt a particular encrypted data key
+          //# (../structures.md#encrypted-data-key), OnDecrypt MUST call AWS KMS
+          //# Decrypt (https://docs.aws.amazon.com/kms/latest/APIReference/
+          //# API_Decrypt.html) with the configured AWS KMS client.
+
+            //= compliance/framework/aws-kms/aws-kms-mrk-keyring.txt#2.8
+            //= type=implication
+            //# When calling AWS KMS Decrypt
+            //# (https://docs.aws.amazon.com/kms/latest/APIReference/
+            //# API_Decrypt.html), the keyring MUST call with a request constructed
+            //# as follows:
+          && var DecryptResponse := Last(client.History.Decrypt).output.value;
+          //= compliance/framework/aws-kms/aws-kms-mrk-keyring.txt#2.8
+          //= type=implication
+          //# If the response does satisfies these requirements then OnDecrypt MUST
+          //# do the following with the response:
+          && output.value.materials.plaintextDataKey == DecryptResponse.Plaintext
+
+
+
+    {
+      var materials := input.materials;
+      var suite := input.materials.algorithmSuite;
+
+      :- Need(
+        Materials.DecryptionMaterialsWithoutPlaintextDataKey(materials),
+        Types.AwsCryptographicMaterialProvidersException( message := "Keyring received decryption materials that already contain a plaintext data key."));
+
+      //= compliance/framework/aws-kms/aws-kms-mrk-keyring.txt#2.8
+      //# The set of encrypted data keys MUST first be filtered to match this
+      //# keyring's configuration.
+      var filter := new OnDecryptEncryptedDataKeyFilter(awsKmsArn);
+      var edksToAttempt :- FilterWithResult(filter, input.encryptedDataKeys);
+
+      :- Need(0 < |edksToAttempt|,
+        Types.AwsCryptographicMaterialProvidersException(
+          message := "Unable to decrypt data key: No Encrypted Data Keys found to match."));
+
+      //= compliance/framework/aws-kms/aws-kms-mrk-keyring.txt#2.8
+      //# For each encrypted data key in the filtered set, one at a time, the
+      //# OnDecrypt MUST attempt to decrypt the data key.
+      //# If this attempt
+      //# results in an error, then these errors MUST be collected.
+      var decryptClosure: DecryptSingleEncryptedDataKey := new DecryptSingleEncryptedDataKey(
+        materials,
+        client,
+        awsKmsKey,
+        grantTokens
+      );
+
+      // assert client.Modifies <= Modifies;
+      // assert decryptClosure.Modifies <= Modifies;
+      //= compliance/framework/aws-kms/aws-kms-mrk-keyring.txt#2.8
+      //# If the response does not satisfies these requirements then an error
+      //# MUST be collected and the next encrypted data key in the filtered set
+      //# MUST be attempted.
+      var outcome, attempts := ReduceToSuccess(
+        decryptClosure,
+        edksToAttempt
+      );
+
+      var SealedDecryptionMaterials :- outcome
+        .MapFailure(errors => Types.Collection( list := errors));
+
+      assert decryptClosure.Ensures(Last(attempts).input, Success(SealedDecryptionMaterials), DropLast(attempts));
+
+      return Success(Types.OnDecryptOutput(
+        materials := SealedDecryptionMaterials
+      ));
+    }
+  }
+
+  class OnDecryptEncryptedDataKeyFilter
+    extends DeterministicActionWithResult<Types.EncryptedDataKey, bool, Types.Error>
+  {
+    const awsKmsKey: AwsKmsIdentifier
+    function Modifies(): set<object> {{}}
+
+    constructor(awsKmsKey: AwsKmsIdentifier) {
+      this.awsKmsKey := awsKmsKey;
+    }
+
+    predicate Ensures(
+      edk: Types.EncryptedDataKey,
+      res: Result<bool, Types.Error>
+    )
+    {
+      && (
+          && res.Success?
+          && res.value
+        ==>
+          edk.keyProviderId == PROVIDER_ID)
+    }
+
+    method Invoke(edk: Types.EncryptedDataKey)
+      returns (res: Result<bool, Types.Error>)
+      ensures Ensures(edk, res)
+    {
+
+      if edk.keyProviderId != PROVIDER_ID {
+        return Success(false);
+      }
+
+      if !UTF8.ValidUTF8Seq(edk.keyProviderInfo) {
+        // The Keyring produces UTF8 keyProviderInfo.
+        // If an `aws-kms` encrypted data key's keyProviderInfo is not UTF8
+        // this is an error, not simply an EDK to filter out.
+        return Failure(
+          Types.AwsCryptographicMaterialProvidersException( message := "Invalid AWS KMS encoding, provider info is not UTF8."));
+      }
+
+      var keyId :- UTF8
+        .Decode(edk.keyProviderInfo)
+        .MapFailure(WrapStringToError);
+      //= compliance/framework/aws-kms/aws-kms-mrk-keyring.txt#2.8
+      //# *  The provider info MUST be a valid AWS KMS ARN (aws-kms-key-
+      //# arn.md#a-valid-aws-kms-arn) with a resource type of "key" or
+      //# OnDecrypt MUST fail.
+      var arn :- ParseAwsKmsArn(keyId).MapFailure(WrapStringToError);
+
+      //= compliance/framework/aws-kms/aws-kms-mrk-keyring.txt#2.8
+      //# *  The the function AWS KMS MRK Match for Decrypt (aws-kms-mrk-match-
+      //# for-decrypt.md#implementation) called with the configured AWS KMS
+      //# key identifier and the provider info MUST return "true".
+      return Success(AwsKmsMrkMatchForDecrypt(
+        awsKmsKey,
+        AwsKmsArnIdentifier(arn)
+      ));
+    }
+  }
+
+  class DecryptSingleEncryptedDataKey
+    extends ActionWithResult<
+      Types.EncryptedDataKey,
+      Materials.SealedDecryptionMaterials,
+      Types.Error>
+  {
+    const materials: Materials.DecryptionMaterialsPendingPlaintextDataKey
+    const client: KMS.IKeyManagementServiceClient
+    const awsKmsKey: AwsKmsIdentifierString
+    const grantTokens: KMS.GrantTokenList
+
+    constructor(
+      materials: Materials.DecryptionMaterialsPendingPlaintextDataKey,
+      client: KMS.IKeyManagementServiceClient,
+      awsKmsKey: AwsKmsIdentifierString,
+      grantTokens: KMS.GrantTokenList
+    )
+      requires client.ValidState()
+      ensures
+      && this.materials == materials
+      && this.client == client
+      && this.awsKmsKey == awsKmsKey
+      && this.grantTokens == grantTokens
+      ensures Invariant()
+    {
+      this.materials := materials;
+      this.client := client;
+      this.awsKmsKey := awsKmsKey;
+      this.grantTokens := grantTokens;
+      Modifies := client.Modifies;
+    }
+
+    predicate Invariant()
+      reads Modifies
+      decreases Modifies
+    {
+      && client.ValidState()
+      && client.Modifies == Modifies
+    }
+
+    predicate Ensures(
+      edk: Types.EncryptedDataKey,
+      res: Result<Materials.SealedDecryptionMaterials, Types.Error>,
+      attempts : seq<ActionInvoke<Types.EncryptedDataKey, Result<Materials.SealedDecryptionMaterials, Types.Error>>>
+    )
+      reads Modifies
+      decreases Modifies
+    {
+      && (res.Success?
+      ==>
+        && Invariant()
+        && KMS.IsValid_CiphertextType(edk.ciphertext)
+        && var maybeStringifiedEncCtx := StringifyEncryptionContext(materials.encryptionContext);
+        && maybeStringifiedEncCtx.Success?
+        && 0 < |client.History.Decrypt|
+        && KMS.DecryptRequest(
+            KeyId := Option.Some(awsKmsKey),
+            CiphertextBlob :=  edk.ciphertext,
+            EncryptionContext := Option.Some(maybeStringifiedEncCtx.Extract()),
+            GrantTokens := Option.Some(grantTokens),
+            EncryptionAlgorithm := Option.None()
+        ) == Last(client.History.Decrypt).input
+        && Last(client.History.Decrypt).output.Success?
+        && Last(client.History.Decrypt).output.value.Plaintext.Some?
+        && Last(client.History.Decrypt).output.value.Plaintext
+          == res.value.plaintextDataKey
+        && Materials.DecryptionMaterialsTransitionIsValid(materials, res.value))
+    }
+
+    method Invoke(
+      edk: Types.EncryptedDataKey,
+      ghost attemptsState: seq<ActionInvoke<Types.EncryptedDataKey, Result<Materials.SealedDecryptionMaterials, Types.Error>>>
+    )
+      returns (res: Result<Materials.SealedDecryptionMaterials, Types.Error>)
+      requires Invariant()
+      decreases Modifies
+      modifies Modifies
+      ensures Invariant()
+      ensures Ensures(edk, res, attemptsState)
+    {
+      :- Need(KMS.IsValid_CiphertextType(edk.ciphertext),
+        Types.AwsCryptographicMaterialProvidersException( message := "Ciphertext length invalid"));
+      var stringifiedEncCtx :- StringifyEncryptionContext(materials.encryptionContext);
+      var decryptRequest := KMS.DecryptRequest(
+        KeyId := Option.Some(awsKmsKey),
+        CiphertextBlob := edk.ciphertext,
+        EncryptionContext := Option.Some(stringifiedEncCtx),
+        GrantTokens := Option.Some(grantTokens),
+        EncryptionAlgorithm := Option.None()
+      );
+
+      var maybeDecryptResponse := client.Decrypt(decryptRequest);
+      var decryptResponse :- maybeDecryptResponse
+        .MapFailure(e => Types.ComAmazonawsKms( ComAmazonawsKms := e ));
+      var suite := materials.algorithmSuite;
+      :- Need(
+        && decryptResponse.KeyId.Some?
+        && decryptResponse.KeyId.value == awsKmsKey
+        && decryptResponse.Plaintext.Some?
+        && AlgorithmSuites.GetEncryptKeyLength(suite) as nat == |decryptResponse.Plaintext.value|
+        , Types.AwsCryptographicMaterialProvidersException( message := "Invalid response from KMS Decrypt"));
+
+      var result :- Materials.DecryptionMaterialsAddDataKey(materials, decryptResponse.Plaintext.value);
+      return Success(result);
+    }
+  }
+
+}
