AwsCryptographicMaterialProviders/src/Keyrings/AwsKms/AwsKmsMrkMatchForDecrypt.dfy
@@ -1,0 +1,91 @@
+// Copyright Amazon.com Inc. or its affiliates. All Rights Reserved.
+// SPDX-License-Identifier: Apache-2.0
+
+include "AwsKmsArnParsing.dfy"
+
+module  AwsKmsMrkMatchForDecrypt {
+  import opened StandardLibrary
+  import opened Wrappers
+  import opened Seq
+  import opened AwsKmsArnParsing
+
+  //= compliance/framework/aws-kms/aws-kms-mrk-match-for-decrypt.txt#2.5
+  //= type=implication
+  //# The caller MUST provide:
+  //# *  2 AWS KMS key identifiers 
+  predicate method AwsKmsMrkMatchForDecrypt(
+    configuredAwsKmsIdentifier: AwsKmsIdentifier,
+    messageAwsKmsIdentifer: AwsKmsIdentifier
+  ) {
+    if (configuredAwsKmsIdentifier == messageAwsKmsIdentifer) then true
+    else
+      match (messageAwsKmsIdentifer, configuredAwsKmsIdentifier) {
+        case (
+          AwsKmsArnIdentifier(configuredAwsKmsArn),
+          AwsKmsArnIdentifier(messageAwsKmsArn)
+        ) =>
+          if !IsMultiRegionAwsKmsArn(configuredAwsKmsArn) || !IsMultiRegionAwsKmsArn(messageAwsKmsArn) then false
+          else
+            && messageAwsKmsArn.partition == configuredAwsKmsArn.partition
+            && messageAwsKmsArn.service   == configuredAwsKmsArn.service
+            && messageAwsKmsArn.account   == configuredAwsKmsArn.account
+            && messageAwsKmsArn.resource  == configuredAwsKmsArn.resource
+        case (_,_) => false
+      }
+  }
+
+  lemma AwsKmsMrkMatchForDecryptCorrect(config: string, message: string)
+    //= compliance/framework/aws-kms/aws-kms-mrk-match-for-decrypt.txt#2.5
+    //= type=implication
+    //# If both identifiers are identical, this function MUST return "true".
+    ensures
+      var c := ParseAwsKmsIdentifier(config);
+      var m := ParseAwsKmsIdentifier(message);
+      && config == message
+      && c.Success?
+      && m.Success?
+    ==>
+      AwsKmsMrkMatchForDecrypt(c.value, m.value)
+    //= compliance/framework/aws-kms/aws-kms-mrk-match-for-decrypt.txt#2.5
+    //= type=implication
+    //# Otherwise if either input is not identified as a multi-Region key
+    //# (aws-kms-key-arn.md#identifying-an-aws-kms-multi-region-key), then
+    //# this function MUST return "false".
+    ensures
+      var c := ParseAwsKmsArn(config);
+      var m := ParseAwsKmsArn(message);
+      && config != message
+      && c.Success?
+      && m.Success?
+      && IsMultiRegionAwsKmsArn(c.value) != IsMultiRegionAwsKmsArn(m.value)
+    ==>
+      !AwsKmsMrkMatchForDecrypt(
+        AwsKmsArnIdentifier(c.value), 
+        AwsKmsArnIdentifier(m.value)
+      );
+    //= compliance/framework/aws-kms/aws-kms-mrk-match-for-decrypt.txt#2.5
+    //= type=implication
+    //# Otherwise if both inputs are
+    //# identified as a multi-Region keys (aws-kms-key-arn.md#identifying-an-
+    //# aws-kms-multi-region-key), this function MUST return the result of
+    //# comparing the "partition", "service", "accountId", "resourceType",
+    //# and "resource" parts of both ARN inputs.
+    ensures
+      var c := ParseAwsKmsArn(config);
+      var m := ParseAwsKmsArn(message);
+      && c.Success?
+      && m.Success?
+      && IsMultiRegionAwsKmsArn(c.value)
+      && IsMultiRegionAwsKmsArn(m.value)
+    ==>
+      AwsKmsMrkMatchForDecrypt(
+        AwsKmsArnIdentifier(c.value),
+        AwsKmsArnIdentifier(m.value)
+      ) == (
+        && m.value.partition == c.value.partition
+        && m.value.service   == c.value.service
+        && m.value.account   == c.value.account
+        && m.value.resource  == c.value.resource
+      );
+  {}
+}
