AwsCryptographicMaterialProviders/src/Keyrings/AwsKms/AwsKmsUtils.dfy
@@ -1,0 +1,147 @@
+// Copyright Amazon.com Inc. or its affiliates. All Rights Reserved.
+// SPDX-License-Identifier: Apache-2.0
+
+include "../../../Model/AwsCryptographyMaterialProvidersTypes.dfy"
+include "AwsKmsArnParsing.dfy"
+
+module AwsKmsUtils {
+  import opened Wrappers
+  import opened UInt = StandardLibrary.UInt
+  import Types = AwsCryptographyMaterialProvidersTypes
+  import KMS = Types.ComAmazonawsKmsTypes
+  import AwsKmsArnParsing
+  import UTF8
+
+  // TODO: These EncryptionContext methods can be removed once we move to UTF8 strings
+  function method StringifyEncryptionContext(utf8EncCtx: Types.EncryptionContext):
+    (res: Result<KMS.EncryptionContextType, Types.Error>)
+  {
+    if |utf8EncCtx| == 0 then Success(map[])
+    else
+      var stringifyResults: map<UTF8.ValidUTF8Bytes, Result<(string, string), Types.Error>> :=
+        map utf8Key | utf8Key in utf8EncCtx.Keys :: utf8Key := StringifyEncryptionContextPair(utf8Key, utf8EncCtx[utf8Key]);
+      if exists r | r in stringifyResults.Values :: r.Failure?
+        then Failure(
+          Types.AwsCryptographicMaterialProvidersException( message := "Encryption context contains invalid UTF8")
+        )
+      else
+        assert forall r | r in stringifyResults.Values :: r.Success?;
+        // TODO state that UTF8.Decode is injective so we don't need this
+        var stringKeysUnique := forall k, k' | k in stringifyResults && k' in stringifyResults
+          :: k != k' ==> stringifyResults[k].value.0 != stringifyResults[k'].value.0;
+        if !stringKeysUnique then Failure(Types.AwsCryptographicMaterialProvidersException(
+          message := "Encryption context keys are not unique"))  // this should never happen...
+        else Success(map r | r in stringifyResults.Values :: r.value.0 := r.value.1)
+  }
+
+  function method StringifyEncryptionContextPair(utf8Key: UTF8.ValidUTF8Bytes, utf8Value: UTF8.ValidUTF8Bytes):
+    (res: Result<(string, string), Types.Error>)
+    ensures (UTF8.Decode(utf8Key).Success? && UTF8.Decode(utf8Value).Success?) <==> res.Success?
+  {
+    var key :- UTF8
+      .Decode(utf8Key)
+      .MapFailure(WrapStringToError);
+    var value :- UTF8
+      .Decode(utf8Value)
+      .MapFailure(WrapStringToError);
+
+    Success((key, value))
+  }
+
+  function method WrapStringToError(e: string)
+    :(ret: Types.Error)
+  {
+    Types.AwsCryptographicMaterialProvidersException( message := e )
+  }
+
+  /*
+   * Returns whether the given client is configured to talk to the given region,
+   * or None if the underlying AWS SDK implementation does not support querying the configuration.
+   *
+   * Useful for MRKs where we need to check whether our client can decrypt an MRK.
+   */
+  function method {:extern "RegionMatch"} RegionMatch(
+    client: KMS.IKeyManagementServiceClient,
+    region: string
+  ): Option<bool>
+
+
+  function method ValidateKmsKeyId(keyId: string)
+    : (res: Result<(), Types.Error>)
+    ensures res.Success? ==>
+      && AwsKmsArnParsing.ParseAwsKmsIdentifier(keyId).Success?
+      && UTF8.IsASCIIString(keyId)
+      && 0 < |keyId| <= AwsKmsArnParsing.MAX_AWS_KMS_IDENTIFIER_LENGTH
+  {
+    var _ :- AwsKmsArnParsing.ParseAwsKmsIdentifier(keyId).MapFailure(WrapStringToError);
+
+    :- Need(UTF8.IsASCIIString(keyId),
+      Types.AwsCryptographicMaterialProvidersException(
+        message := "Key identifier is not ASCII"));
+    :- Need(0 < |keyId| <= AwsKmsArnParsing.MAX_AWS_KMS_IDENTIFIER_LENGTH,
+      Types.AwsCryptographicMaterialProvidersException(
+        message := "Key identifier is too long"));
+    Success(())
+  }
+
+  function method GetValidGrantTokens(grantTokens: Option<Types.GrantTokenList>)
+    : (res: Result<Types.GrantTokenList, Types.Error>)
+    ensures res.Success? ==>
+      var tokens := res.value;
+      && 0 <= |tokens| <= 10
+      && forall token | token in tokens :: 1 <= |token| <= 8192
+    ensures res.Success? && grantTokens.Some? ==> res.value == grantTokens.value
+  {
+    var tokens: Types.GrantTokenList := grantTokens.UnwrapOr([]);
+    :- Need(0 <= |tokens| <= 10,
+      Types.AwsCryptographicMaterialProvidersException(
+        message := "Grant token list can have no more than 10 tokens"));
+    :- Need(forall token | token in tokens :: 1 <= |token| <= 8192,
+      Types.AwsCryptographicMaterialProvidersException(
+        message := "Grant token list contains a grant token with invalid length"));
+    Success(tokens)
+  }
+
+  function method ParseKeyNamespaceAndName(keyNamespace: string, keyName: string)
+    : (res: Result<(UTF8.ValidUTF8Bytes, UTF8.ValidUTF8Bytes), Types.Error>)
+    ensures res.Success? ==>
+      var (namespace, name) := res.value;
+      && |namespace| < UINT16_LIMIT
+      && |name| < UINT16_LIMIT
+  {
+    var namespace :- UTF8.Encode(keyNamespace)
+      .MapFailure(e => Types.AwsCryptographicMaterialProvidersException(
+        message := "Key namespace could not be UTF8-encoded" + e ));
+    :- Need(|namespace| < UINT16_LIMIT,
+      Types.AwsCryptographicMaterialProvidersException(
+        message := "Key namespace too long"));
+
+    var name :- UTF8.Encode(keyName)
+      .MapFailure(e => Types.AwsCryptographicMaterialProvidersException(
+        message := "Key name could not be UTF8-encoded" + e ));
+    :- Need(|name| < UINT16_LIMIT,
+      Types.AwsCryptographicMaterialProvidersException(
+        message := "Key name too long"));
+
+    Success((namespace, name))
+  }
+
+  function method ValidateDiscoveryFilter(filter: Types.DiscoveryFilter)
+    : (res: Result<(), Types.Error>)
+    ensures res.Success? ==>
+      && |filter.accountIds| > 0
+      && (forall accountId | accountId in filter.accountIds :: |accountId| > 0)
+      && |filter.partition| > 0
+  {
+    :- Need(|filter.accountIds| > 0,
+      Types.AwsCryptographicMaterialProvidersException(
+        message := "Discovery filter must have at least one account ID"));
+    :- Need(forall accountId | accountId in filter.accountIds :: |accountId| > 0,
+      Types.AwsCryptographicMaterialProvidersException(
+        message := "Discovery filter account IDs cannot be blank"));
+    :- Need(|filter.partition| > 0,
+      Types.AwsCryptographicMaterialProvidersException(
+        message := "Discovery filter partition cannot be blank"));
+    Success(())
+  }
+}
