AwsCryptographicMaterialProviders/src/Keyrings/AwsKms/MrkAwareDiscoveryMultiKeyring.dfy
@@ -1,0 +1,132 @@
+// Copyright Amazon.com Inc. or its affiliates. All Rights Reserved.
+// SPDX-License-Identifier: Apache-2.0
+include "../../../../libraries/src/Collections/Sequences/Seq.dfy"
+
+include "../../../Model/AwsCryptographyMaterialProvidersTypes.dfy"
+include "../MultiKeyring.dfy"
+include "AwsKmsArnParsing.dfy"
+include "AwsKmsMrkAreUnique.dfy"
+include "AwsKmsMrkDiscoveryKeyring.dfy"
+include "AwsKmsUtils.dfy"
+include "../../AlgorithmSuites.dfy"
+
+module MrkAwareDiscoveryMultiKeyring {
+  import opened Wrappers
+  import Seq
+  import Types = AwsCryptographyMaterialProvidersTypes 
+  import KMS = Types.ComAmazonawsKmsTypes
+  import MultiKeyring
+  import AwsKmsArnParsing
+  import AwsKmsMrkAreUnique
+  import AwsKmsMrkDiscoveryKeyring
+  import opened AwsKmsUtils
+
+  //= compliance/framework/aws-kms/aws-kms-mrk-multi-keyrings.txt#2.6
+  //= type=implication
+  //# The caller MUST provide:
+  //#*  A set of Region strings
+  //#*  An optional discovery filter that is an AWS partition and a set of
+  //#   AWS accounts
+  //#*  An optional method that can take a region string and return an AWS
+  //#   KMS client e.g. a regional client supplier
+  //#*  An optional list of AWS KMS grant tokens
+  method MrkAwareDiscoveryMultiKeyring(
+    regions: seq<string>,
+    discoveryFilter: Option<Types.DiscoveryFilter>,
+    clientSupplier: Types.IClientSupplier,
+    grantTokens: Option<KMS.GrantTokenList>
+  )
+    returns (
+      output: Result<MultiKeyring.MultiKeyring, Types.Error>
+    )
+    requires clientSupplier.ValidState()
+    modifies clientSupplier.Modifies
+    ensures output.Success? ==>
+    && output.value.ValidState()
+    && fresh(output.value)
+    && fresh(output.value.History)
+    && fresh(output.value.Modifies - clientSupplier.Modifies)
+
+    ensures
+      //= compliance/framework/aws-kms/aws-kms-mrk-multi-keyrings.txt#2.6
+      //= type=implication
+      //# If an empty set of Region is provided this function MUST fail.
+      || |regions| == 0
+      //= compliance/framework/aws-kms/aws-kms-mrk-multi-keyrings.txt#2.6
+      //= type=implication
+      //# If
+      //# any element of the set of regions is null or an empty string this
+      //# function MUST fail.
+      || (exists r | r in regions :: r == "")
+    ==>
+      output.Failure?
+
+    //= compliance/framework/aws-kms/aws-kms-mrk-multi-keyrings.txt#2.6
+    //= type=implication
+    //# Then a Multi-Keyring (../multi-keyring.md#inputs) MUST be initialize
+    //# by using this set of discovery keyrings as the child keyrings
+    //# (../multi-keyring.md#child-keyrings).
+    //# This Multi-Keyring MUST be
+    //# this functions output.
+    ensures
+      && output.Success?
+    ==>
+      && output.value.generatorKeyring.None?
+      && |regions| == |output.value.childKeyrings|
+      && forall i | 0 <= i < |regions|
+      ::
+        && var k: Types.IKeyring := output.value.childKeyrings[i];
+        && k is AwsKmsMrkDiscoveryKeyring.AwsKmsMrkDiscoveryKeyring
+        && var c := k as AwsKmsMrkDiscoveryKeyring.AwsKmsMrkDiscoveryKeyring;
+        //= compliance/framework/aws-kms/aws-kms-mrk-multi-keyrings.txt#2.6
+        //= type=implication
+        //# Then a set of AWS KMS MRK Discovery Keyring (aws-kms-mrk-discovery-
+        //# keyring.md) MUST be created for each AWS KMS client by initializing
+        //# each keyring with
+        //#*  The AWS KMS client
+        //#*  The input discovery filter
+        //#*  The input AWS KMS grant tokens
+        && c.region == regions[i]
+        && (discoveryFilter.Some? ==> c.discoveryFilter == discoveryFilter)
+        && (grantTokens.Some? ==> c.grantTokens == grantTokens.value)
+  {
+    :- Need(|regions| > 0, Types.AwsCryptographicMaterialProvidersException(
+        message := "No regions passed."));
+    :- Need(Seq.IndexOfOption(regions, "").None?, Types.AwsCryptographicMaterialProvidersException(
+        message := "Empty string is not a valid region."));
+
+    var children : seq<AwsKmsMrkDiscoveryKeyring.AwsKmsMrkDiscoveryKeyring> := [];
+
+    for i := 0 to |regions|
+        invariant |regions[..i]| == |children|
+        invariant fresh(MultiKeyring.GatherModifies(None, children) - clientSupplier.Modifies)
+        invariant forall i | 0 <= i < |children|
+        ::
+          && children[i].region == regions[i]
+          && (discoveryFilter.Some? ==> children[i].discoveryFilter == discoveryFilter)
+          && (grantTokens.Some? ==> children[i].grantTokens == grantTokens.value)
+          && children[i].ValidState()
+      {
+        var region := regions[i];
+        //= compliance/framework/aws-kms/aws-kms-mrk-multi-keyrings.txt#2.6
+        //# A set of AWS KMS clients MUST be created by calling regional client
+        //# supplier for each region in the input set of regions.
+        var client :- clientSupplier.GetClient(Types.GetClientInput(region := region));
+        var keyring := new AwsKmsMrkDiscoveryKeyring.AwsKmsMrkDiscoveryKeyring(
+          client,
+          region,
+          discoveryFilter,
+          grantTokens.UnwrapOr([])
+        );
+        // Order is important
+        children := children + [keyring];
+      }
+
+    var keyring := new MultiKeyring.MultiKeyring(
+      None(),
+      children
+    );
+
+    return Success(keyring);
+  }
+}
