AwsCryptographicMaterialProviders/src/Keyrings/RawRSAKeyring.dfy
@@ -1,0 +1,396 @@
+// Copyright Amazon.com Inc. or its affiliates. All Rights Reserved.
+// SPDX-License-Identifier: Apache-2.0
+
+include "../Keyring.dfy"
+include "../Materials.dfy"
+include "../AlgorithmSuites.dfy"
+include "../../../src/StandardLibrary/String.dfy"
+include "../AlgorithmSuites.dfy"
+include "../Materials.dfy"
+include "../../Model/AwsCryptographyMaterialProvidersTypes.dfy"
+include "../../../libraries/src/Collections/Sequences/Seq.dfy"
+
+module RawRSAKeyring {
+  import opened StandardLibrary
+  import opened UInt = StandardLibrary.UInt
+  import opened String = StandardLibrary.String
+  import opened Wrappers
+  import Types = AwsCryptographyMaterialProvidersTypes
+  import Crypto = AwsCryptographyPrimitivesTypes
+  import Aws.Cryptography.Primitives
+  import Keyring
+  import Materials
+  import opened AlgorithmSuites
+  import Random
+  import RSAEncryption
+  import UTF8
+  import Seq
+
+  //= compliance/framework/raw-rsa-keyring.txt#2.5.2
+  //= type=TODO
+  //# The raw RSA keyring SHOULD support loading PEM
+  //# encoded X.509 SubjectPublicKeyInfo structures
+  //# (https://tools.ietf.org/html/rfc5280#section-4.1) as public keys.
+
+  class RawRSAKeyring
+    extends Keyring.VerifiableInterface, Types.IKeyring
+  {
+    const cryptoPrimitives: Primitives.AtomicPrimitivesClient
+
+    predicate ValidState()
+      ensures ValidState() ==> History in Modifies
+    {
+      && History in Modifies
+      && cryptoPrimitives.Modifies <= Modifies
+      && History !in cryptoPrimitives.Modifies
+      && cryptoPrimitives.ValidState()
+    }
+
+    const keyNamespace: UTF8.ValidUTF8Bytes
+    const keyName: UTF8.ValidUTF8Bytes
+    const publicKey: Option<seq<uint8>>
+    const privateKey: Option<seq<uint8>>
+    const paddingScheme: Crypto.RSAPaddingMode
+
+    //= compliance/framework/raw-rsa-keyring.txt#2.5
+    //= type=implication
+    //# On keyring initialization, the caller MUST provide the following:
+    //#*  Key Namespace (./keyring-interface.md#key-namespace)
+    //#*  Key Name (./keyring-interface.md#key-name)
+    //#*  Padding Scheme (Section 2.5.1)
+    //#*  Public Key (Section 2.5.2) and/or Private Key (Section 2.5.3)
+    constructor (
+      namespace: UTF8.ValidUTF8Bytes,
+      name: UTF8.ValidUTF8Bytes,
+
+      //= compliance/framework/raw-rsa-keyring.txt#2.5.2
+      //= type=TODO
+      //# The public key MUST follow the RSA specification for public keys
+      //# (Section 2.4.2).
+      // NOTE: section 2.4.2 is a lie,
+      // See https://datatracker.ietf.org/doc/html/rfc8017#section-3.1 instead
+      // NOTE: A sequence of uint8 is NOT how a public key is stored according to the RFC linked, though it is how the libraries we use define them
+      publicKey: Option<seq<uint8>>,
+
+      //= compliance/framework/raw-rsa-keyring.txt#2.5.3
+      //= type=TODO
+      //# The private key MUST follow the RSA specification for private keys
+      //# (Section 2.4.2).
+      // NOTE: section 2.4.2 is a lie,
+      // See https://datatracker.ietf.org/doc/html/rfc8017#section-3.2 instead
+      // NOTE: A sequence of uint8s is NOT how a public key is stored according to the RFC linked, though it is how the libraries we use define them
+      privateKey: Option<seq<uint8>>,
+
+      //= compliance/framework/raw-rsa-keyring.txt#2.5.3
+      //= type=TODO
+      //# The
+      //# private key SHOULD contain all Chinese Remainder Theorem (CRT)
+      //# components (public exponent, prime factors, CRT exponents, and CRT
+      //# coefficient).
+      // NOTE: What? Shouldn't the above be on the Cryptographic library?
+      // i.e.: BouncyCastle, pyca, etc.?
+
+      //= compliance/framework/raw-rsa-keyring.txt#2.5.1
+      //= type=implication
+      //# This value MUST correspond with one of the supported padding schemes
+      //# (Section 2.5.1.1).
+      paddingScheme: Crypto.RSAPaddingMode,
+      cryptoPrimitives: Primitives.AtomicPrimitivesClient
+    )
+      requires |namespace| < UINT16_LIMIT
+      requires |name| < UINT16_LIMIT
+      requires cryptoPrimitives.ValidState()
+      ensures this.keyNamespace == namespace
+      ensures this.keyName == name
+      ensures this.paddingScheme == paddingScheme
+      ensures this.publicKey == publicKey
+      ensures this.privateKey == privateKey
+      ensures ValidState() && fresh(History) && fresh(Modifies - cryptoPrimitives.Modifies)
+    {
+      this.keyNamespace := namespace;
+      this.keyName := name;
+      this.paddingScheme := paddingScheme;
+      this.publicKey := publicKey;
+      this.privateKey := privateKey;
+
+      this.cryptoPrimitives := cryptoPrimitives;
+
+      History := new Types.IKeyringCallHistory();
+      Modifies := { History } + cryptoPrimitives.Modifies;
+    }
+
+    predicate OnEncryptEnsuresPublicly(input: Types.OnEncryptInput, output: Result<Types.OnEncryptOutput, Types.Error>) {true}
+
+    //= compliance/framework/raw-rsa-keyring.txt#2.6.1
+    //= type=implication
+    //# OnEncrypt MUST take encryption materials (structures.md#encryption-
+    //# materials) as input.
+    method OnEncrypt'(input: Types.OnEncryptInput)
+      returns (output: Result<Types.OnEncryptOutput, Types.Error>)
+      requires ValidState()
+      modifies Modifies - {History}
+      decreases Modifies - {History}
+      ensures ValidState()
+      ensures OnEncryptEnsuresPublicly(input, output)
+      ensures unchanged(History)
+      ensures
+        output.Success?
+      ==>
+        && Materials.ValidEncryptionMaterialsTransition(
+          input.materials,
+          output.value.materials
+        )
+
+     //= compliance/framework/raw-rsa-keyring.txt#2.6.1
+     //= type=implication
+     //# OnEncrypt MUST fail if this keyring does not have a specified public
+     //# key (Section 2.5.2).
+     ensures
+       this.publicKey.None? || |this.publicKey.Extract()| == 0
+     ==>
+       output.Failure?
+
+     //= compliance/framework/raw-rsa-keyring.txt#2.6.1
+     //= type=implication
+     //# If the encryption materials (structures.md#encryption-materials) do
+     //# not contain a plaintext data key, OnEncrypt MUST generate a random
+     //# plaintext data key and set it on the encryption materials
+     //# (structures.md#encryption-materials).
+     ensures
+       && input.materials.plaintextDataKey.None?
+       && output.Success?
+     ==>
+       output.value.materials.plaintextDataKey.Some?
+
+     //= compliance/framework/raw-rsa-keyring.txt#2.6.1
+     //= type=implication
+     //# If RSA encryption was successful, OnEncrypt MUST return the input
+     //# encryption materials (structures.md#encryption-materials), modified
+     //# in the following ways:
+     //#*  The encrypted data key list has a new encrypted data key added,
+     //#   constructed as follows:
+     ensures
+       && output.Success?
+     ==>
+       |output.value.materials.encryptedDataKeys| == |input.materials.encryptedDataKeys| + 1
+
+     //= compliance/framework/raw-rsa-keyring.txt#2.6.1
+     //= type=implication
+     //# The keyring MUST NOT derive a public key from a
+     //# specified private key (Section 2.5.3).
+     // NOTE: Attempting to proove this by stating that a Keyring
+     // without a public key but with a private key will not encrypt
+     ensures
+       this.privateKey.Some? && this.publicKey.None?
+     ==>
+       output.Failure?
+    {
+      :- Need(
+        this.publicKey.Some? && |this.publicKey.Extract()| > 0,
+        Types.AwsCryptographicMaterialProvidersException(
+          message := "A RawRSAKeyring without a public key cannot provide OnEncrypt"));
+
+      var materials := input.materials;
+      var suite := materials.algorithmSuite;
+
+      // While this may be an unnecessary operation, it is more legiable to generate
+      // and then maybe use this new plain text datakey then generate it in the if statement
+      var generateBytesResult := cryptoPrimitives
+        .GenerateRandomBytes(Crypto.GenerateRandomBytesInput(length := GetEncryptKeyLength(suite)));
+      var newPlaintextDataKey :- generateBytesResult.MapFailure(e => Types.AwsCryptographyPrimitives(AwsCryptographyPrimitives := e));
+
+      //= compliance/framework/raw-rsa-keyring.txt#2.6.1
+      //# If the encryption materials (structures.md#encryption-materials) do
+      //# not contain a plaintext data key, OnEncrypt MUST generate a random
+      //# plaintext data key and set it on the encryption materials
+      //# (structures.md#encryption-materials).
+      var plaintextDataKey :=
+        if materials.plaintextDataKey.Some? && |materials.plaintextDataKey.Extract()| > 0
+        then materials.plaintextDataKey.value
+        else newPlaintextDataKey;
+
+      //= compliance/framework/raw-rsa-keyring.txt#2.6.1
+      //# The keyring MUST attempt to encrypt the plaintext data key in the
+      //# encryption materials (structures.md#encryption-materials) using RSA.
+      //# The keyring performs RSA encryption (Section 2.4.2) with the
+      //# following specifics:
+      var RSAEncryptOutput := cryptoPrimitives.RSAEncrypt(Crypto.RSAEncryptInput(
+        //= compliance/framework/raw-rsa-keyring.txt#2.6.1
+        //#*  This keyring's padding scheme (Section 2.5.1.1) is the RSA padding
+        //#   scheme.
+        padding := paddingScheme,
+
+        //= compliance/framework/raw-rsa-keyring.txt#2.6.1
+        //#*  This keyring's public key (Section 2.5.2) is the RSA public key.
+        publicKey := publicKey.Extract(),
+
+        //= compliance/framework/raw-rsa-keyring.txt#2.6.1
+        //#*  The plaintext data key is the plaintext input to RSA encryption.
+        plaintext := plaintextDataKey
+      ));
+
+      var ciphertext :- RSAEncryptOutput.MapFailure(e => Types.AwsCryptographyPrimitives(e));
+
+      //= compliance/framework/raw-rsa-keyring.txt#2.6.1
+      //# If RSA encryption was successful, OnEncrypt MUST return the input
+      //# encryption materials (structures.md#encryption-materials), modified
+      //# in the following ways:
+      //#*  The encrypted data key list has a new encrypted data key added,
+      //#   constructed as follows:
+      var edk: Types.EncryptedDataKey := Types.EncryptedDataKey(
+
+        //= compliance/framework/raw-rsa-keyring.txt#2.6.1
+        //#  -  The key provider ID (structures.md#key-provider-id) field is
+        //#     this keyring's key namespace (keyring-interface.md#key-
+        //#     namespace).
+        keyProviderId := this.keyNamespace,
+
+        //= compliance/framework/raw-rsa-keyring.txt#2.6.1
+        //#  -  The key provider information (structures.md#key-provider-
+        //#     information) field is this keyring's key name (keyring-
+        //#     interface.md#key-name).
+        keyProviderInfo := this.keyName,
+
+        //= compliance/framework/raw-rsa-keyring.txt#2.6.1
+        //#  -  The ciphertext (structures.md#ciphertext) field is the
+        //#     ciphertext output by the RSA encryption of the plaintext data
+        //#     key.
+        ciphertext := ciphertext
+      );
+
+      var returnMaterials :- if materials.plaintextDataKey.None? then
+        Materials.EncryptionMaterialAddDataKey(materials, plaintextDataKey, [edk])
+      else
+        Materials.EncryptionMaterialAddEncryptedDataKeys(materials, [edk]);
+      return Success(Types.OnEncryptOutput(materials := returnMaterials));
+    }
+
+    predicate OnDecryptEnsuresPublicly(input: Types.OnDecryptInput, output: Result<Types.OnDecryptOutput, Types.Error>){true}
+
+    //= compliance/framework/raw-rsa-keyring.txt#2.6.2
+    //= type=implication
+    //# OnDecrypt MUST take decryption materials (structures.md#decryption-
+    //# materials) and a list of encrypted data keys
+    //# (structures.md#encrypted-data-key) as input.
+    method OnDecrypt'(input: Types.OnDecryptInput)
+      returns (output: Result<Types.OnDecryptOutput, Types.Error>)
+      requires ValidState()
+      modifies Modifies - {History}
+      decreases Modifies - {History}
+      ensures ValidState()
+      ensures OnDecryptEnsuresPublicly(input, output)
+      ensures unchanged(History)
+      ensures output.Success?
+      ==>
+        && Materials.DecryptionMaterialsTransitionIsValid(
+          input.materials,
+          output.value.materials
+        )
+
+      //= compliance/framework/raw-rsa-keyring.txt#2.6.2
+      //= type=implication
+      //# OnDecrypt MUST fail if this keyring does not have a specified private
+      //# key (Section 2.5.3).
+      ensures
+        privateKey.None? || |privateKey.Extract()| == 0
+      ==>
+        output.Failure?
+
+      //= compliance/framework/raw-rsa-keyring.txt#2.6.2
+      //= type=implication
+      //# If the decryption materials already contain a plaintext data key, the
+      //# keyring MUST fail and MUST NOT modify the decryption materials
+      //# (structures.md#decryption-materials).
+      ensures
+        input.materials.plaintextDataKey.Some?
+      ==>
+        output.Failure?
+    {
+      :- Need(
+        this.privateKey.Some? && |this.privateKey.Extract()| > 0,
+        Types.AwsCryptographicMaterialProvidersException(
+          message := "A RawRSAKeyring without a private key cannot provide OnEncrypt"));
+
+      var materials := input.materials;
+      :- Need(
+        Materials.DecryptionMaterialsWithoutPlaintextDataKey(materials),
+        Types.AwsCryptographicMaterialProvidersException(
+          message := "Keyring received decryption materials that already contain a plaintext data key."));
+
+      var errors: seq<Types.Error> := [];
+      //= compliance/framework/raw-rsa-keyring.txt#2.6.2
+      //# The keyring MUST attempt to decrypt the input encrypted data keys, in
+      //# list order, until it successfully decrypts one.
+      for i := 0 to |input.encryptedDataKeys|
+        invariant |errors| == i
+      {
+        if ShouldDecryptEDK(input.encryptedDataKeys[i]) {
+          var edk := input.encryptedDataKeys[i];
+          var decryptResult := cryptoPrimitives.RSADecrypt(Crypto.RSADecryptInput(
+            padding := paddingScheme,
+            privateKey := privateKey.Extract(),
+            cipherText := edk.ciphertext
+          ));
+
+          //= compliance/framework/raw-rsa-keyring.txt#2.6.2
+          //# If any decryption succeeds, this keyring MUST immediately return the
+          //# input decryption materials (structures.md#decryption-materials),
+          //# modified in the following ways:
+          if decryptResult.Success? {
+            //= compliance/framework/raw-rsa-keyring.txt#2.6.2
+            //#*  The output of RSA decryption is set as the decryption material's
+            //#   plaintext data key.
+            var returnMaterials :- Materials.DecryptionMaterialsAddDataKey(
+              materials,
+              decryptResult.Extract()
+            );
+            return Success(Types.OnDecryptOutput(materials := returnMaterials));
+          } else {
+            errors := errors + [Types.AwsCryptographyPrimitives(decryptResult.error)];
+          }
+        } else {
+          errors := errors + [Types.AwsCryptographicMaterialProvidersException( message :=
+            "EncryptedDataKey "
+            + Base10Int2String(i)
+            + " did not match RSAKeyring. ")
+          ];
+        }
+      }
+      //= compliance/framework/raw-rsa-keyring.txt#2.6.2
+      //# If no decryption succeeds, the keyring MUST fail and MUST NOT modify
+      //# the decryption materials (structures.md#decryption-materials).
+      return Failure(Types.Collection(list := errors));
+    }
+
+    predicate method ShouldDecryptEDK(edk: Types.EncryptedDataKey)
+      //= compliance/framework/raw-rsa-keyring.txt#2.6.2
+      //= type=implication
+      //# For each encrypted data key, the keyring MUST attempt to decrypt the
+      //# encrypted data key into plaintext using RSA if and only if the
+      //# following is true:
+      ensures
+        //= compliance/framework/raw-rsa-keyring.txt#2.6.2
+        //= type=implication
+        //#*  The encrypted data key's key provider information
+        //#   (structures.md#key-provider-information). has a value equal to
+        //#   this keyring's key name (keyring-interface.md#key-name).
+        && edk.keyProviderInfo == this.keyName
+
+        //= compliance/framework/raw-rsa-keyring.txt#2.6.2
+        //= type=implication
+        //#*  The encrypted data key's key provider ID (structures.md#key-
+        //#   provider-id) has a value equal to this keyring's key namespace
+        //#   (keyring-interface.md#key-namespace).
+        && edk.keyProviderId == this.keyNamespace
+
+        && |edk.ciphertext| > 0
+      ==>
+        true
+    {
+      && UTF8.ValidUTF8Seq(edk.keyProviderInfo)
+      && edk.keyProviderInfo == this.keyName
+      && edk.keyProviderId == this.keyNamespace
+      && |edk.ciphertext| > 0
+    }
+  }
+}
