AwsCryptographicMaterialProviders/Model/identifiers.smithy
@@ -1,0 +1,70 @@
+namespace aws.cryptography.materialProviders
+
+/////////////
+// Commitment
+
+@enum([
+  {
+    name: "FORBID_ENCRYPT_ALLOW_DECRYPT",
+    value: "FORBID_ENCRYPT_ALLOW_DECRYPT",
+  },
+  {
+    name: "REQUIRE_ENCRYPT_ALLOW_DECRYPT",
+    value: "REQUIRE_ENCRYPT_ALLOW_DECRYPT",
+  },
+  {
+    name: "REQUIRE_ENCRYPT_REQUIRE_DECRYPT",
+    value: "REQUIRE_ENCRYPT_REQUIRE_DECRYPT",
+  },
+])
+string ESDKCommitmentPolicy
+
+union CommitmentPolicy {
+  ESDK: ESDKCommitmentPolicy
+}
+
+//////////
+// Padding
+
+// Values come from: https://github.com/awslabs/aws-encryption-sdk-specification/blob/master/framework/raw-rsa-keyring.md#supported-padding-schemes
+@enum([
+  {
+    name: "PKCS1",
+    value: "PKCS1",
+  },
+  {
+    name: "OAEP_SHA1_MGF1",
+    value: "OAEP_SHA1_MGF1",
+  },
+  {
+    name: "OAEP_SHA256_MGF1",
+    value: "OAEP_SHA256_MGF1",
+  },
+  {
+    name: "OAEP_SHA384_MGF1",
+    value: "OAEP_SHA384_MGF1",
+  },
+  {
+    name: "OAEP_SHA512_MGF1",
+    value: "OAEP_SHA512_MGF1",
+  },
+])
+string PaddingScheme
+
+//////////////////////////
+// AES wrapping algorithms
+@enum([
+  {
+    name: "ALG_AES128_GCM_IV12_TAG16",
+    value: "ALG_AES128_GCM_IV12_TAG16",
+  },
+  {
+    name: "ALG_AES192_GCM_IV12_TAG16",
+    value: "ALG_AES192_GCM_IV12_TAG16",
+  },
+  {
+    name: "ALG_AES256_GCM_IV12_TAG16",
+    value: "ALG_AES256_GCM_IV12_TAG16",
+  },
+])
+string AesWrappingAlg
