AwsCryptographicMaterialProviders/Model/material-provider.smithy
@@ -1,0 +1,64 @@
+namespace aws.cryptography.materialProviders
+
+/////////////
+// AwsCryptographicMaterialProviders Creation
+@aws.polymorph#localService(
+  sdkId: "MaterialProviders",
+  config: MaterialProvidersConfig,
+)
+service AwsCryptographicMaterialProviders {
+  version: "2021-11-01",
+  resources: [
+    Keyring,
+    CryptographicMaterialsManager,
+    ClientSupplier,
+  ],
+  operations: [
+    // Keyrings
+    CreateAwsKmsKeyring,
+    CreateAwsKmsDiscoveryKeyring,
+    CreateAwsKmsMultiKeyring,
+    CreateAwsKmsDiscoveryMultiKeyring,
+    CreateAwsKmsMrkKeyring,
+    CreateAwsKmsMrkMultiKeyring,
+    CreateAwsKmsMrkDiscoveryKeyring,
+    CreateAwsKmsMrkDiscoveryMultiKeyring,
+    CreateMultiKeyring,
+    CreateRawAesKeyring,
+    CreateRawRsaKeyring,
+
+    // CMMs
+    CreateDefaultCryptographicMaterialsManager,
+
+    // ClientSupplier
+    CreateDefaultClientSupplier,
+
+    // Materials
+    InitializeEncryptionMaterials,
+    InitializeDecryptionMaterials,
+    ValidEncryptionMaterialsTransition,
+    ValidDecryptionMaterialsTransition,
+    EncryptionMaterialsHasPlaintextDataKey,
+    DecryptionMaterialsWithPlaintextDataKey,
+
+    // AlgorithmSuiteInfo
+    GetAlgorithmSuiteInfo,
+    ValidAlgorithmSuiteInfo,
+
+    // Commitment
+    ValidateCommitmentPolicyOnEncrypt,
+    ValidateCommitmentPolicyOnDecrypt,
+  ],
+  errors: [AwsCryptographicMaterialProvidersException],
+}
+
+structure MaterialProvidersConfig {}
+
+///////////////////
+// Errors
+
+@error("client")
+structure AwsCryptographicMaterialProvidersException {
+  @required
+  message: String,
+}
