AwsCryptographicMaterialProviders/Model/structures.smithy
@@ -1,0 +1,77 @@
+namespace aws.cryptography.materialProviders
+
+use aws.polymorph#dafnyUtf8Bytes
+
+@dafnyUtf8Bytes
+string Utf8Bytes
+
+///////////////////////////////////
+// Encryption Materials 
+
+// In the future, we have several improvements we can consider here:
+//   1. Model these materials structures as resources, in order to move towards "smarter"
+//      materials. This would allow us to tightly define the valid interactions with
+//      materials and prevent dangerous or unexpected uses of them. 
+//   2. Use different materials structures for keyrings and CMMs. These live at
+//      different layers of the library and have different needs and responsibilities,
+//      so we may eventually want to give them each materials specialized to their
+//      purpose.
+// Note that both of these will be breaking changes to any customers building
+// custom implementations of keyrings or CMMs.
+structure EncryptionMaterials {
+  @required
+  algorithmSuite: AlgorithmSuiteInfo,
+
+  @required
+  encryptionContext: EncryptionContext,
+
+  @required
+  encryptedDataKeys: EncryptedDataKeyList,
+
+  plaintextDataKey: Secret,
+
+  signingKey: Secret
+}
+
+structure DecryptionMaterials {
+  @required
+  algorithmSuite: AlgorithmSuiteInfo,
+
+  @required
+  encryptionContext: EncryptionContext,
+
+  plaintextDataKey: Secret,
+
+  verificationKey: Secret
+}
+
+structure EncryptedDataKey {
+  // The spec defines keyProviderId in 2 places,
+  // and, while they are not identical,
+  // they do not disagree.
+  // data-format/message-header.md#encrypted-data-key-entries ::
+  // UTF-8 encoded bytes
+  // framework/keyring-interface.md#key-provider-id ::
+  // The key provider ID MUST be a binary value and SHOULD be equal to a UTF-8 encoding of the key namespace.
+  @required
+  keyProviderId: Utf8Bytes,
+
+  // The key provider info MUST be a binary value and SHOULD be equal to a UTF-8 encoding of the key name.
+  @required
+  keyProviderInfo: Blob,
+
+  @required
+  ciphertext: Blob
+}
+
+list EncryptedDataKeyList {
+  member: EncryptedDataKey
+}
+
+map EncryptionContext {
+  key: Utf8Bytes,
+  value: Utf8Bytes,
+}
+
+@sensitive
+blob Secret
