AwsCryptographicMaterialProviders/Model/suites.smithy
@@ -1,0 +1,142 @@
+namespace aws.cryptography.materialProviders
+
+///////////////////////////////////
+// Algorithm Suites
+
+// For now, the actual properties of algorithm suites are only used by internal
+// components and are not actually customer facing. If and when we make them
+// customer facing, we will need to either model the AlgorithmSuiteProperties
+// as a separate structure (with an associated resource/operation for translating
+// from name to properties) or use more advanced custom traits which allow us to
+// model all properties of the algorithm suite in one structure. 
+@enum([
+  {
+    name: "ALG_AES_128_GCM_IV12_TAG16_NO_KDF",
+    value: "0x0014",
+  },
+  {
+    name: "ALG_AES_192_GCM_IV12_TAG16_NO_KDF",
+    value: "0x0046",
+  },
+  {
+    name: "ALG_AES_256_GCM_IV12_TAG16_NO_KDF",
+    value: "0x0078",
+  },
+  {
+    name: "ALG_AES_128_GCM_IV12_TAG16_HKDF_SHA256",
+    value: "0x0114",
+  },
+  {
+    name: "ALG_AES_192_GCM_IV12_TAG16_HKDF_SHA256",
+    value: "0x0146",
+  },
+  {
+    name: "ALG_AES_256_GCM_IV12_TAG16_HKDF_SHA256",
+    value: "0x0178",
+  },
+  {
+    name: "ALG_AES_128_GCM_IV12_TAG16_HKDF_SHA256_ECDSA_P256",
+    value: "0x0214",
+  },
+  {
+    name: "ALG_AES_192_GCM_IV12_TAG16_HKDF_SHA384_ECDSA_P384",
+    value: "0x0346",
+  },
+  {
+    name: "ALG_AES_256_GCM_IV12_TAG16_HKDF_SHA384_ECDSA_P384",
+    value: "0x0378",
+  },
+  {
+    name: "ALG_AES_256_GCM_HKDF_SHA512_COMMIT_KEY",
+    value: "0x0478",
+  },
+  {
+    name: "ALG_AES_256_GCM_HKDF_SHA512_COMMIT_KEY_ECDSA_P384",
+    value: "0x0578",
+  },
+])
+string ESDKAlgorithmSuiteId
+
+union AlgorithmSuiteId {
+  ESDK: ESDKAlgorithmSuiteId
+}
+
+structure AlgorithmSuiteInfo {
+  @required
+  id: AlgorithmSuiteId,
+  @required
+  binaryId: Blob,
+  @required
+  messageVersion: Integer,
+  @required
+  encrypt: Encrypt,
+  @required
+  kdf: DerivationAlgorithm,
+  @required
+  commitment: DerivationAlgorithm,
+  @required
+  signature: SignatureAlgorithm,
+}
+ 
+union Encrypt {
+  AES_GCM: aws.cryptography.primitives#AES_GCM,
+}
+
+union DerivationAlgorithm {
+  HKDF: HKDF,
+  // We are using both `IDENTITY` and `None` here
+  // to modle the fact that deriving
+  // the data encryption key and the commitment key
+  // MUST be the same.
+  // The specification treats NO_KDF as an identity operation.
+  // So this naming convention mirrors the specification.
+  IDENTITY: IDENTITY,
+  None: None,
+}
+
+union SignatureAlgorithm {
+  ECDSA: ECDSA,
+  None: None
+}
+
+structure HKDF {
+  @required
+  hmac: aws.cryptography.primitives#DigestAlgorithm,
+  @required
+  saltLength: aws.cryptography.primitives#PositiveInteger,
+  @required
+  inputKeyLength: aws.cryptography.primitives#SymmetricKeyLength,
+  @required
+  outputKeyLength: aws.cryptography.primitives#SymmetricKeyLength,
+}
+structure IDENTITY {}
+structure None {}
+
+structure ECDSA {
+  @required
+  curve: aws.cryptography.primitives#ECDSASignatureAlgorithm,
+}
+
+@readonly
+operation GetAlgorithmSuiteInfo {
+  input: GetAlgorithmSuiteInfoInput,
+  output: AlgorithmSuiteInfo,
+}
+
+@aws.polymorph#positional
+structure GetAlgorithmSuiteInfoInput {
+  @required
+  binaryId: Blob
+}
+
+@readonly
+operation ValidAlgorithmSuiteInfo {
+  input: AlgorithmSuiteInfo,
+  errors: [InvalidAlgorithmSuiteInfo]
+}
+
+@error("client")
+structure InvalidAlgorithmSuiteInfo {
+  @required
+  message: String,
+}
